Equivocators composition 3 (#144)
* Equivocators composition with no non-equivocating participant

* Equivocators composition vs Free Composition

* Refactorings

VLSM/Equivocators/Composition/Common.v
@@ -39,8 +39,8 @@ the label, and keeping only the copy of index 1 for each machine.
 Section fully_equivocating_composition.
 
 Context {message : Type}
-  {equiv_index nequiv_index : Type}
-  (index := sum equiv_index nequiv_index)
+  {equiv_index : Type}
+  (index := equiv_index)
   {IndEqDec : EqDecision index}
   (IM : index -> VLSM message)
   (Hbs : forall i : index, has_been_sent_capability (IM i))
@@ -48,38 +48,23 @@ Context {message : Type}
   (X := free_composite_vlsm IM i0)
   .
 
-Local Instance equiv_index_eq_dec : EqDecision equiv_index.
-Proof.
-  intros x y.
-  destruct (decide (inl x = inl y)).
-  - left. inversion e. reflexivity.
-  - right. intro contra. elim n. subst. reflexivity.
-Qed.
-
 Definition equivocator_IM
   (i : index)
   : VLSM message
   :=
-  match i with
-  | inl _ => equivocator_vlsm (IM i)
-  | inr _ => (IM i)
-  end.
+  equivocator_vlsm (IM i).
 
 Lemma equivocator_Hbs
   (i : index)
   :  has_been_sent_capability (equivocator_IM i).
 Proof.
   unfold equivocator_IM.
-  destruct i as [eqv | neqv] eqn:Hi.
-  - apply equivocator_has_been_sent_capability. apply Hbs.
-  - apply Hbs.
+  apply equivocator_has_been_sent_capability. apply Hbs.
 Qed.
 
 Context
   (index_listing : list index)
   (finite_index : Listing index_listing)
-  (equiv_listing := left_listing finite_index)
-  (finite_equiv := left_finite finite_index)
   .
 
 Definition equivocators_no_equivocations_constraint
@@ -106,14 +91,14 @@ Lemma equivocators_initial_state_size
   (is : vstate equivocators_no_equivocations_vlsm)
   (His : vinitial_state_prop equivocators_no_equivocations_vlsm is)
   (eqv : equiv_index)
-  : projT1 (is (inl eqv)) = 0.
+  : projT1 (is eqv) = 0.
 Proof.
-  specialize (His (inl eqv)).
+  specialize (His eqv).
   destruct His as [Hzero His].
   assumption.
 Qed.
 
-Definition equivocators_choice : Type := forall (eqv : equiv_index), MachineDescriptor (IM (inl eqv)).
+Definition equivocators_choice : Type := forall (eqv : equiv_index), MachineDescriptor (IM eqv).
 
 Definition proper_equivocators_choice
   (eqv_choice : equivocators_choice)
@@ -121,7 +106,7 @@ Definition proper_equivocators_choice
   : Prop
   := forall
     (eqv : equiv_index),
-    proper_descriptor (IM (inl eqv)) (eqv_choice eqv) (s (inl eqv)).
+    proper_descriptor (IM eqv) (eqv_choice eqv) (s eqv).
 
 Definition not_equivocating_equivocators_choice
   (eqv_choice : equivocators_choice)
@@ -129,7 +114,7 @@ Definition not_equivocating_equivocators_choice
   : Prop
   := forall
     (eqv : equiv_index),
-    not_equivocating_descriptor (IM (inl eqv)) (eqv_choice eqv) (s (inl eqv)).
+    not_equivocating_descriptor (IM eqv) (eqv_choice eqv) (s eqv).
 
 Lemma not_equivocating_equivocators_choice_proper
   (eqv_choice : equivocators_choice)
@@ -142,7 +127,7 @@ Qed.
 
 Definition zero_choice
   (eqv : equiv_index)
-  : MachineDescriptor (IM (inl eqv))
+  : MachineDescriptor (IM eqv)
   := Existing _ 0 false.
 
 Lemma zero_choice_not_equivocating
@@ -163,62 +148,40 @@ Lemma proper_equivocators_choice_state_update_eqv
   (eqv_choice : equivocators_choice)
   (s : vstate equivocators_free_vlsm)
   (eqv : equiv_index)
-  (si : vstate (equivocator_IM (inl eqv)))
-  (Hsi_proper : proper_descriptor (IM (inl eqv)) (eqv_choice eqv) (s (inl eqv)))
-  (Hproper : proper_equivocators_choice eqv_choice (state_update equivocator_IM s (inl eqv) si))
+  (si : vstate (equivocator_IM eqv))
+  (Hsi_proper : proper_descriptor (IM eqv) (eqv_choice eqv) (s eqv))
+  (Hproper : proper_equivocators_choice eqv_choice (state_update equivocator_IM s eqv si))
   : proper_equivocators_choice eqv_choice s.
 Proof.
   intro eqv'.
   specialize (Hproper eqv').
-  destruct (decide (inl eqv' = inl eqv)).
-  - inversion e. subst. rewrite state_update_eq in Hproper. assumption.
+  destruct (decide (eqv' = eqv)).
+  - subst. rewrite state_update_eq in Hproper. assumption.
   - rewrite state_update_neq in Hproper; assumption.
-Qed.
-
-Lemma proper_equivocators_choice_state_update_neqv
-  (eqv_choice : equivocators_choice)
-  (s : vstate equivocators_free_vlsm)
-  (neqv : nequiv_index)
-  (si : vstate (equivocator_IM (inr neqv)))
-  (Hproper : proper_equivocators_choice eqv_choice (state_update equivocator_IM s (inr neqv) si))
-  : proper_equivocators_choice eqv_choice s.
-Proof.
-  intro eqv.
-  specialize (Hproper eqv).
-  destruct (decide (inl eqv = inr neqv)); try discriminate e.
-  rewrite state_update_neq in Hproper; assumption.
 Qed.
 
 Definition equivocators_state_project
   (eqv_choice : equivocators_choice)
   (s : vstate equivocators_free_vlsm)
-  (i : index)
-  : vstate (IM i)
+  (eqv : index)
+  : vstate (IM eqv)
   :=
-  let si := s i in
-  match i with
-  | inl eqv =>
-    match (eqv_choice eqv) with
-    | NewMachine _ sn => sn
-    | Existing _ j _ =>
-      let (n, bs) := s (inl eqv) in
-      match (le_lt_dec (S n) j) with
-      | right lt_in => bs (of_nat_lt lt_in)
-      | left _ => bs F1
-      end
+  match (eqv_choice eqv) with
+  | NewMachine _ sn => sn
+  | Existing _ j _ =>
+    let (n, bs) := s eqv in
+    match (le_lt_dec (S n) j) with
+    | right lt_in => bs (of_nat_lt lt_in)
+    | left _ => bs F1
     end
-  | inr neqv => s (inr neqv)
   end.
 
 Definition lift_to_equivocators_state
   (s : vstate X)
-  (i : index)
-  : vstate (equivocator_IM i)
+  (eqv : index)
+  : vstate (equivocator_IM eqv)
   :=
-  match i with
-  | inl eqv => mk_singleton_state _ (s (inl eqv))
-  | inr neqv => s (inr neqv)
-  end.
+  mk_singleton_state _ (s eqv).
 
 Lemma lift_initial_to_equivocators_state
   (s : vstate X)
@@ -228,9 +191,7 @@ Proof.
   unfold vinitial_state_prop in *. simpl in *.
   unfold composite_initial_state_prop in *.
   intro i. spec Hs i.
-  destruct i as [eqv | neqv].
-  - split; try assumption. reflexivity.
-  - assumption.
+  split; [reflexivity|assumption].
 Qed.
 
 (**
@@ -240,12 +201,12 @@ to a component:
 Definition equivocators_choice_update
   (s : equivocators_choice)
   (i : equiv_index)
-  (si : MachineDescriptor (IM (inl i)))
+  (si : MachineDescriptor (IM i))
   (j : equiv_index)
-  : MachineDescriptor (IM (inl j))
+  : MachineDescriptor (IM j)
   :=
   match decide (j = i) with
-  | left e => eq_rect_r (fun i => MachineDescriptor (IM (inl i))) si e
+  | left e => eq_rect_r (fun i => MachineDescriptor (IM i)) si e
   | _ => s j
   end.
 
@@ -255,18 +216,18 @@ The next few results describe several properties of the [equivocators_choice_upd
 Lemma equivocators_choice_update_neq
   (s : equivocators_choice)
   (i : equiv_index)
-  (si : MachineDescriptor (IM (inl i)))
+  (si : MachineDescriptor (IM i))
   (j : equiv_index)
   (Hneq : j <> i)
   : equivocators_choice_update s i si j = s j.
 Proof.
-  unfold equivocators_choice_update. destruct (decide (j = i)); try contradiction. reflexivity.
+  unfold equivocators_choice_update. destruct (decide (j = i)); congruence.
 Qed.
 
 Lemma equivocators_choice_update_eq
   (s : equivocators_choice)
   (i : equiv_index)
-  (si : MachineDescriptor (IM (inl i)))
+  (si : MachineDescriptor (IM i))
   : equivocators_choice_update s i si i = si.
 Proof.
   unfold equivocators_choice_update.
@@ -276,7 +237,7 @@ Qed.
 Lemma equivocators_choice_update_id
   (s : equivocators_choice)
   (i : equiv_index)
-  (si : MachineDescriptor (IM (inl i)))
+  (si : MachineDescriptor (IM i))
   (Heq : s i = si)
   : equivocators_choice_update s i si = s.
 Proof.
@@ -290,7 +251,7 @@ Qed.
 Lemma equivocators_choice_update_twice
   (s : equivocators_choice)
   (i : equiv_index)
-  (si si': MachineDescriptor (IM (inl i)))
+  (si si': MachineDescriptor (IM i))
   : equivocators_choice_update (equivocators_choice_update s i si) i si'
   = equivocators_choice_update s i si'.
 Proof.
@@ -298,37 +259,15 @@ Proof.
   intro j.
   destruct (decide (j = i)).
   - subst. rewrite equivocators_choice_update_eq. symmetry. apply equivocators_choice_update_eq.
-  - repeat rewrite equivocators_choice_update_neq; try assumption.
+  - repeat rewrite equivocators_choice_update_neq by assumption.
     reflexivity.
-Qed.
-
-Lemma equivocators_state_project_state_update_neqv
-  (eqv_choice : equivocators_choice)
-  (s : vstate equivocators_free_vlsm)
-  (neqv : nequiv_index)
-  (sneqv : vstate (equivocator_IM (inr neqv)))
-  : equivocators_state_project eqv_choice (state_update equivocator_IM s (inr neqv) sneqv)
-  = state_update IM (equivocators_state_project eqv_choice s) (inr neqv) sneqv.
-Proof.
-  apply functional_extensionality_dep.
-  intro i.
-  unfold equivocators_state_project.
-  unfold state_update.
-  destruct i as [ieqv|ineqv]
-  ; match goal with
-    |- context [decide ?d] => destruct (decide d)
-    end; [discriminate e|reflexivity|..|reflexivity].
-  inversion e. subst.
-  unfold eq_rect_r.
-  elim_eq_rect.
-  reflexivity.
 Qed.
 
 Lemma equivocators_state_project_state_update_eqv
   (eqv_choice : equivocators_choice)
   (s : vstate equivocators_free_vlsm)
   (eqv : equiv_index)
-  (seqv : vstate (equivocator_IM (inl eqv)))
+  (seqv : vstate (equivocator_IM eqv))
   : let si :=  match eqv_choice eqv with
     | NewMachine _ sn => sn
     | Existing _ i _ =>
@@ -337,17 +276,16 @@ Lemma equivocators_state_project_state_update_eqv
       | right l => projT2 seqv (of_nat_lt l)
       end
     end in
-  equivocators_state_project eqv_choice (state_update equivocator_IM s (inl eqv) seqv)
-  = state_update IM (equivocators_state_project eqv_choice s) (inl eqv) si.
+  equivocators_state_project eqv_choice (state_update equivocator_IM s eqv seqv)
+  = state_update IM (equivocators_state_project eqv_choice s) eqv si.
 Proof.
   apply functional_extensionality_dep.
-  intro i.
+  intro ieqv.
   unfold equivocators_state_project.
   unfold state_update.
-  destruct i as [ieqv|ineqv]
-  ; match goal with
+  match goal with
     |- context [decide ?d] => destruct (decide d)
-    end; [|reflexivity|discriminate e|reflexivity].
+    end; [|reflexivity].
   inversion e. subst. unfold eq_rect_r.
   elim_eq_rect. unfold eq_rect.
   destruct seqv as (n, bs).
@@ -361,15 +299,14 @@ Lemma equivocators_initial_state_project
   (Heqv : proper_equivocators_choice eqv_choice es)
   : vinitial_state_prop X (equivocators_state_project eqv_choice es).
 Proof.
-  intro n. specialize (Hes n).
+  intro eqv. specialize (Hes eqv).
   unfold equivocator_IM in Hes.
   unfold equivocators_state_project.
-  destruct n as [eqv|neqv]; try assumption.
   specialize (Heqv eqv).
-  destruct (eqv_choice eqv) as [sn | i fi]; try assumption.
+  destruct (eqv_choice eqv) as [sn | i fi]; [assumption|].
   destruct Hes as [Hzero Hes].
-  destruct (es (inl eqv)) as (n, bs). simpl in Heqv.
-  destruct (le_lt_dec (S n) i). { lia. }
+  destruct (es eqv) as (n, bs). simpl in Heqv.
+  destruct (le_lt_dec (S n) i); [lia|].
   simpl in *.
   subst. assert (Hi: i = 0) by lia. subst.
   assumption.
@@ -380,18 +317,17 @@ Lemma equivocators_initial_message
   (Hem : vinitial_message_prop equivocators_free_vlsm m)
   : vinitial_message_prop X m.
 Proof.
-  destruct Hem as [i [emi Hem]].
-  exists i.
+  destruct Hem as [eqv [emi Hem]].
+  exists eqv.
   unfold equivocator_IM in emi.
-  destruct i as [eqv | neqv]; exists emi; assumption.
+  exists emi. assumption.
 Qed.
 
-Local Tactic Notation "unfold_transition"  hyp(H) :=
-  ( unfold transition in H; unfold equivocator_vlsm in H
-  ; unfold Common.equivocator_vlsm in H
-  ; unfold mk_vlsm in H; unfold machine in H
-  ; unfold projT2 in H; unfold equivocator_vlsm_machine in H
-  ; unfold equivocator_transition in H).
+Local Tactic Notation "unfold_transition"  hyp(Ht) :=
+  ( unfold transition in Ht; unfold equivocator_IM in Ht;
+  unfold equivocator_vlsm in Ht; unfold mk_vlsm in Ht;
+  unfold machine in Ht; unfold projT2 in Ht;
+  unfold equivocator_vlsm_machine in Ht; unfold equivocator_transition in Ht). 
 
 Lemma equivocators_protocol_state_project
   (es : vstate equivocators_no_equivocations_vlsm)
@@ -412,7 +348,7 @@ Proof.
       intros.
       specialize (equivocators_initial_state_project _ His eqv_choice Heqv) as HisX.
       remember (equivocators_state_project eqv_choice is) as isX.
-      replace isX with (proj1_sig (exist _ _ HisX)); try reflexivity.
+      change isX with (proj1_sig (exist _ _ HisX)).
       exists None.
       apply protocol_initial_state.
   - split.
@@ -424,584 +360,524 @@ Proof.
       intros.
       specialize (equivocators_initial_state_project _ His eqv_choice Heqv) as HisX.
       remember (equivocators_state_project eqv_choice is) as isX.
-      replace isX with (proj1_sig (exist _ _ HisX)); try reflexivity.
+      change isX with (proj1_sig (exist _ _ HisX)).
       exists None.
       apply protocol_initial_state.
   - specialize (IHHes1 s _om JMeq_refl). apply proj2 in IHHes1.
     specialize (IHHes2 _s om0 JMeq_refl). apply proj1 in IHHes2.
     simpl in x.
-    destruct l as (i, li).
-    destruct (vtransition (equivocator_IM i) li (s i, om0)) as (si', om') eqn:Ht.
+    destruct l as (eqv, li).
+    destruct (vtransition (equivocator_IM eqv) li (s eqv, om0)) as (si', om') eqn:Ht.
     inversion x. subst es om. clear x.
     destruct Hv as [Hv _]. simpl in Hv.
     specialize (protocol_generated X) as Hgen.
-    destruct i as [ieqv | ineqv].
-    * destruct li as (li, di).
-      specialize (Hgen (existT _ (inl ieqv) li)) as Hgen_om'.
-      simpl in Hv. unfold vvalid in Hv. simpl in Hv.
-      simpl in Ht. unfold vtransition in Ht. unfold_transition Ht.
-      unfold snd in Ht.
-      destruct di as [sn | i fi].
-      -- destruct Hv as [Hsn Hv].
-        subst om0.
-        inversion Ht. subst. clear Ht.
-        split; try assumption.
-        intros eqv_choice Heqv.
-        destruct (s (inl ieqv)) as (n, bs) eqn:Hsieqv.
-        destruct (eqv_choice ieqv) as [sieqv | iieqv fieqv] eqn:Hieqv.
-        ++ assert (Heqvs : proper_equivocators_choice eqv_choice s).
+    destruct li as (li, di).
+    specialize (Hgen (existT _ eqv li)) as Hgen_om'.
+    simpl in Hv. unfold vvalid in Hv. simpl in Hv.
+    simpl in Ht. unfold vtransition in Ht.
+    unfold_transition Ht.
+    unfold snd in Ht.
+    destruct di as [sn | i fi].
+    -- destruct Hv as [Hsn Hv].
+      subst om0.
+      inversion Ht. subst. clear Ht.
+      split; [assumption|].
+      intros eqv_choice Heqv.
+      destruct (s eqv) as (n, bs) eqn:Hsieqv.
+      destruct (eqv_choice eqv) as [sieqv | iieqv fieqv] eqn:Hieqv.
+      ++ assert (Heqvs : proper_equivocators_choice eqv_choice s).
+        { intro eqv'. specialize (Heqv eqv').
+          simpl in *.
+          destruct (decide (eqv' = eqv))
+          ; [|rewrite state_update_neq in Heqv; assumption].
+          inversion e. subst. rewrite state_update_eq in Heqv.
+          rewrite Hieqv in *. simpl in Heqv. assumption.
+        }
+        specialize (IHHes1 _ Heqvs).
+        replace
+          (equivocators_state_project eqv_choice
+          (state_update equivocator_IM s eqv
+             (equivocator_state_extend (IM eqv)
+                (existT (fun n0 : nat => t (S n0) -> vstate (IM eqv)) n bs)
+                sn)))
+          with (equivocators_state_project eqv_choice s)
+          ; [assumption|].
+        apply functional_extensionality_dep.
+        intros eqv'. unfold equivocators_state_project.
+        destruct (eqv_choice eqv') eqn:Heqv'; [reflexivity|].
+        destruct (decide (eqv' = eqv)).
+        --- subst.
+          rewrite state_update_eq.
+          unfold equivocator_state_extend.
+          rewrite Hsieqv.
+          specialize (Heqvs eqv).
+          rewrite Heqv' in Heqvs. simpl in Heqvs.
+          rewrite Hsieqv in Heqvs. simpl in Heqvs.
+          destruct (le_lt_dec (S n) n0); [lia|].
+          destruct (le_lt_dec (S (S n)) n0); [lia|].
+          rewrite to_nat_of_nat.
+          destruct (nat_eq_dec n0 (S n)); [lia|].
+          f_equal. apply of_nat_ext.
+        --- rewrite state_update_neq by assumption. reflexivity.
+      ++ specialize (Heqv eqv) as Heqvi. unfold proper_descriptor in Heqvi.
+        rewrite Hieqv in Heqvi. rewrite state_update_eq in Heqvi.
+        simpl in Heqvi.
+        destruct (nat_eq_dec iieqv (S n)).
+        ** subst.
+          pose (equivocators_choice_update eqv_choice eqv (NewMachine _ sn)) as eqv_choice'.
+          specialize (IHHes1 eqv_choice').
+          spec IHHes1.
+          { intro eqv'. spec Heqv eqv'.
+            destruct (decide (eqv' = eqv)).
+            - subst.
+              unfold eqv_choice'.
+              rewrite equivocators_choice_update_eq.
+              assumption.
+            - rewrite state_update_neq in Heqv by assumption.
+              unfold eqv_choice'.
+              rewrite equivocators_choice_update_neq by assumption.
+              assumption.
+          }
+          replace
+            (equivocators_state_project eqv_choice
+            (state_update equivocator_IM s eqv
+               (equivocator_state_extend (IM eqv)
+                  (existT (fun n0 : nat => t (S n0) -> vstate (IM eqv)) n bs)
+                  sn)))
+            with
+              (equivocators_state_project eqv_choice' s)
+          ; [assumption|].
+          apply functional_extensionality_dep.
+          intro i.
+          unfold equivocators_state_project at 1. unfold eqv_choice'.
+          rewrite equivocators_state_project_state_update_eqv.
+          destruct (decide (i = eqv)).
+          --- subst. repeat rewrite state_update_eq.
+            rewrite equivocators_choice_update_eq.
+            rewrite Hieqv. unfold equivocator_state_extend.
+            unfold projT1. unfold projT2.
+            destruct (le_lt_dec (S (S n)) (S n)); [lia|].
+            rewrite to_nat_of_nat.
+            destruct (nat_eq_dec (S n) (S n)); congruence.
+          --- repeat rewrite state_update_neq; [|assumption].
+            unfold equivocators_state_project.
+            rewrite equivocators_choice_update_neq; congruence.
+        ** assert (Heqvs : proper_equivocators_choice eqv_choice s).
           { intro eqv'. specialize (Heqv eqv').
             simpl in *.
-            destruct (decide (inl eqv' = inl ieqv))
-            ; try (rewrite state_update_neq in Heqv; assumption).
-            inversion e. subst. rewrite state_update_eq in Heqv.
+            destruct (decide (eqv' = eqv))
+            ; [| rewrite state_update_neq in Heqv; assumption].
+            subst. rewrite state_update_eq in Heqv.
+            rewrite Hieqv in *. simpl in Heqv. simpl.
+            rewrite Hsieqv. simpl. lia.
+          }
+          specialize (IHHes1 _ Heqvs).
+          replace
+            (equivocators_state_project eqv_choice
+            (state_update equivocator_IM s eqv
+               (equivocator_state_extend (IM eqv)
+                  (existT (fun n0 : nat => t (S n0) -> vstate (IM eqv)) n bs)
+                  sn)))
+            with (equivocators_state_project eqv_choice s)
+          ; [assumption|].
+          apply functional_extensionality_dep.
+          intros eqv'. unfold equivocators_state_project.
+          destruct (eqv_choice eqv') eqn:Heqv'; [reflexivity|].
+          destruct (decide (eqv' = eqv))
+          ; [|rewrite state_update_neq; [reflexivity|assumption]].
+          subst.
+          rewrite state_update_eq.
+          unfold equivocator_state_extend.
+          rewrite Hsieqv.
+          specialize (Heqvs eqv).
+          rewrite Heqv' in Heqvs. simpl in Heqvs.
+          rewrite Hsieqv in Heqvs. simpl in Heqvs.
+          destruct (le_lt_dec (S n) n1); [lia|].
+          destruct (le_lt_dec (S (S n)) n1); [lia|].
+          rewrite to_nat_of_nat.
+          destruct (nat_eq_dec n1 (S n)); [lia|].
+          f_equal. apply of_nat_ext.
+    -- destruct Hv as [Hi Hv].
+      destruct (le_lt_dec (S (projT1 (s eqv))) i); [lia|].
+      unfold fst in Ht.
+      destruct (vtransition (IM eqv) li (projT2 (s eqv) (of_nat_lt l), om0))
+        as (sieqv', om0') eqn:Ht'.
+      destruct fi eqn:Hfi; inversion Ht; subst si' om'; clear Ht.
+      ++ pose
+        (equivocators_choice_update
+          (fun eqv => NewMachine _ (proj1_sig (vs0 (IM (eqv)))))
+          eqv (Existing _ i false)
+        ) as eqv_choice'.
+        specialize (IHHes1 eqv_choice') as Hs_om'.
+        spec Hs_om'.
+        { intro eqv'. unfold eqv_choice'.
+          destruct (decide (eqv' = eqv)).
+          + subst. rewrite equivocators_choice_update_eq. assumption.
+          + rewrite equivocators_choice_update_neq by assumption.
+            simpl. destruct (vs0 (IM (eqv'))). assumption.
+        }
+        destruct Hs_om' as [_oms Hs_om'].
+        destruct IHHes2 as [_som0 Hom0].
+        specialize (Hgen_om' _ _ Hs_om' _ _ Hom0).
+        spec Hgen_om'.
+        { split; [|exact I].
+          unfold free_composite_valid.
+          unfold equivocators_state_project.
+          unfold eqv_choice'.
+          rewrite equivocators_choice_update_eq.
+          destruct (s eqv) as (nieqv, bsieqv).
+          simpl in Hi.
+          destruct (le_lt_dec (S nieqv) i); [lia|].
+          replace (of_nat_lt l0) with (of_nat_lt Hi) by apply of_nat_ext.
+          assumption.
+        }
+        remember (equivocators_state_project eqv_choice' s) as sp.
+        simpl in Hgen_om'.
+        subst sp. unfold equivocators_state_project at 1 in Hgen_om'.
+        unfold eqv_choice' at 1 in Hgen_om'.
+        rewrite equivocators_choice_update_eq in Hgen_om'.
+        destruct (s eqv) as (nieqv, bsieqv) eqn:Hsieqv.
+        simpl in Hi.
+        destruct (le_lt_dec (S nieqv) i); [lia|].
+        simpl in l. simpl in Ht'.
+        replace (of_nat_lt l) with (of_nat_lt Hi) in * by apply of_nat_ext.
+        clear l.
+        replace (of_nat_lt l0) with (of_nat_lt Hi) in * by apply of_nat_ext.
+        clear l0.
+        rewrite Ht' in Hgen_om'.
+        split; [eexists _; apply Hgen_om'|].
+        intros eqv_choice Heqv.
+        unfold_transition Hgen_om'.
+        destruct (eqv_choice eqv) as [sieqv | iieqv fieqv] eqn:Hieqv.
+        ** assert (Heqvs : proper_equivocators_choice eqv_choice s).
+          { intro eqv'. specialize (Heqv eqv').
+            simpl in *.
+            destruct (decide (eqv' = eqv))
+            ; [| rewrite state_update_neq in Heqv; assumption].
+            subst. rewrite state_update_eq in Heqv.
             rewrite Hieqv in *. simpl in Heqv. assumption.
           }
           specialize (IHHes1 _ Heqvs).
           replace
             (equivocators_state_project eqv_choice
-            (state_update equivocator_IM s (inl ieqv)
-               (equivocator_state_extend (IM (inl ieqv))
-                  (existT (fun n0 : nat => t (S n0) -> vstate (IM (inl ieqv))) n bs)
-                  sn)))
+            (state_update equivocator_IM s eqv
+               (equivocator_state_extend (IM eqv)
+                  (existT (fun n : nat => t (S n) -> vstate (IM eqv)) nieqv bsieqv) sieqv')))
             with (equivocators_state_project eqv_choice s)
-            ; try assumption.
+            ; [assumption|].
           apply functional_extensionality_dep.
-          intros [eqv'|neqv']; unfold equivocators_state_project.
-          ** destruct (eqv_choice eqv') eqn:Heqv'; try reflexivity.
-            destruct (decide (inl eqv' = inl ieqv)).
-            --- inversion e. subst.
-              rewrite state_update_eq.
-              unfold equivocator_state_extend.
-              rewrite Hsieqv.
-              specialize (Heqvs ieqv).
-              rewrite Heqv' in Heqvs. simpl in Heqvs.
-              rewrite Hsieqv in Heqvs. simpl in Heqvs.
-              destruct (le_lt_dec (S n) n0). { lia. }
-              destruct (le_lt_dec (S (S n)) n0). { lia. }
-              rewrite to_nat_of_nat.
-              destruct (nat_eq_dec n0 (S n)). { lia. }
-              f_equal. apply of_nat_ext.
-            --- rewrite state_update_neq; try assumption. reflexivity.
-          ** rewrite state_update_neq; try reflexivity.
-            intro contra. discriminate contra.
-        ++ specialize (Heqv ieqv) as Heqvi. unfold proper_descriptor in Heqvi.
+          intros eqv'. unfold equivocators_state_project.
+          destruct (eqv_choice eqv') eqn:Heqv'; [reflexivity|].
+          destruct (decide (eqv' = eqv))
+          ; [|rewrite state_update_neq; [reflexivity|assumption]].
+          inversion e. subst.
+          rewrite state_update_eq.
+          unfold equivocator_state_extend.
+          rewrite Hsieqv.
+          specialize (Heqvs eqv).
+          rewrite Heqv' in Heqvs. simpl in Heqvs.
+          rewrite Hsieqv in Heqvs. simpl in Heqvs.
+          destruct (le_lt_dec (S nieqv) n); [lia|].
+          destruct (le_lt_dec (S (S nieqv)) n); [lia|].
+          rewrite to_nat_of_nat.
+          destruct (nat_eq_dec n (S nieqv)); [lia|].
+          f_equal. apply of_nat_ext.
+        ** specialize (Heqv eqv) as Heqvi. unfold proper_descriptor in Heqvi.
           rewrite Hieqv in Heqvi. rewrite state_update_eq in Heqvi.
           simpl in Heqvi.
-          destruct (nat_eq_dec iieqv (S n)).
-          ** subst.
-            pose (equivocators_choice_update eqv_choice ieqv (NewMachine _ sn)) as eqv_choice'.
-            specialize (IHHes1 eqv_choice').
+          destruct (nat_eq_dec iieqv (S nieqv)).
+          --- subst.
+            pose (equivocators_choice_update eqv_choice eqv (Existing _ i false)) as eqv_choice''.
+            specialize (IHHes1 eqv_choice'').
             spec IHHes1.
             { intro eqv'. spec Heqv eqv'.
-              destruct (decide (inl eqv' = inl ieqv)).
-              - inversion e. subst.
-                unfold eqv_choice'.
+              destruct (decide (eqv' = eqv)).
+              - subst.
+                unfold eqv_choice''.
                 rewrite equivocators_choice_update_eq.
+                simpl. rewrite Hsieqv.
                 assumption.
-              - rewrite state_update_neq in Heqv; try assumption.
-                unfold eqv_choice'.
-                assert (n' : eqv' <> ieqv) by (intro contra; subst; elim n0; reflexivity).
+              - rewrite state_update_neq in Heqv; [|assumption].
+                unfold eqv_choice''.
                 rewrite equivocators_choice_update_neq; assumption.
             }
+            specialize (Hgen (existT _ eqv li)).
+            destruct IHHes1 as [_oms' Hs].
+            specialize (Hgen _ _ Hs _ _ Hom0).
+            spec Hgen.
+            { split; [|exact I].
+              unfold free_composite_valid. unfold vvalid. simpl in Hv.
+              replace (equivocators_state_project eqv_choice'' s eqv) with (bsieqv (of_nat_lt Hi)); try assumption.
+              unfold eqv_choice''.
+              unfold equivocators_state_project.
+              rewrite equivocators_choice_update_eq.
+              rewrite Hsieqv.
+              destruct (le_lt_dec (S nieqv) i); [lia|].
+              f_equal. apply of_nat_ext.
+            }
+            unfold transition in Hgen.
+            unfold X in Hgen at 2. unfold free_composite_vlsm in Hgen.
+            unfold composite_vlsm in Hgen.
+            unfold mk_vlsm in Hgen.
+            unfold machine in Hgen.
+            unfold projT2 in Hgen.
+            unfold composite_vlsm_machine in Hgen.
+            unfold composite_transition in Hgen.
+            unfold equivocators_state_project at 1 in Hgen.
+            unfold eqv_choice'' in Hgen.
+            rewrite equivocators_choice_update_eq in Hgen.
+            rewrite Hsieqv in Hgen.
+            destruct (le_lt_dec (S nieqv) i); [lia|].
+            replace (of_nat_lt l) with (of_nat_lt Hi) in * by apply of_nat_ext.
+            rewrite Ht' in Hgen.
+            exists om0'.
             replace
               (equivocators_state_project eqv_choice
-              (state_update equivocator_IM s (inl ieqv)
-                 (equivocator_state_extend (IM (inl ieqv))
-                    (existT (fun n0 : nat => t (S n0) -> vstate (IM (inl ieqv))) n bs)
-                    sn)))
-              with
-                (equivocators_state_project eqv_choice' s)
-            ; try assumption.
+              (state_update equivocator_IM s eqv
+                 (equivocator_state_extend (IM eqv)
+                    (existT (fun n : nat => t (S n) -> vstate (IM eqv)) nieqv bsieqv) sieqv')))
+              with (state_update IM
+              (equivocators_state_project
+                 (equivocators_choice_update eqv_choice eqv (Existing (IM eqv) i false)) s)
+              eqv sieqv')
+              ; [assumption|].
             apply functional_extensionality_dep.
-            intro i.
-            unfold equivocators_state_project at 1. unfold eqv_choice'.
+            intro i'.
             rewrite equivocators_state_project_state_update_eqv.
-            destruct (decide (i = inl ieqv)).
-            --- subst. repeat rewrite state_update_eq.
-              rewrite equivocators_choice_update_eq.
+            destruct (decide (i' = eqv)).
+            +++ subst. repeat rewrite state_update_eq.
               rewrite Hieqv. unfold equivocator_state_extend.
               unfold projT1. unfold projT2.
-              destruct (le_lt_dec (S (S n)) (S n)). { lia. }
+              destruct (le_lt_dec (S (S nieqv)) (S nieqv)); [lia|].
               rewrite to_nat_of_nat.
-              destruct (nat_eq_dec (S n) (S n)); congruence.
-            --- repeat rewrite state_update_neq; try assumption.
+              destruct (nat_eq_dec (S nieqv) (S nieqv)); [reflexivity|].
+              elim n. reflexivity.
+            +++ repeat rewrite state_update_neq by assumption.
               unfold equivocators_state_project.
-              destruct i; try reflexivity.
-              rewrite equivocators_choice_update_neq ; congruence.
-          ** assert (Heqvs : proper_equivocators_choice eqv_choice s).
+              rewrite equivocators_choice_update_neq; [reflexivity|].
+              assumption.
+          --- assert (Heqvs : proper_equivocators_choice eqv_choice s).
             { intro eqv'. specialize (Heqv eqv').
               simpl in *.
-              destruct (decide (inl eqv' = inl ieqv))
-              ; try (rewrite state_update_neq in Heqv; assumption).
-              inversion e. subst. rewrite state_update_eq in Heqv.
+              destruct (decide (eqv' = eqv))
+              ; [|rewrite state_update_neq in Heqv; assumption].
+              subst. rewrite state_update_eq in Heqv.
               rewrite Hieqv in *. simpl in Heqv. simpl.
               rewrite Hsieqv. simpl. lia.
             }
             specialize (IHHes1 _ Heqvs).
             replace
               (equivocators_state_project eqv_choice
-              (state_update equivocator_IM s (inl ieqv)
-                 (equivocator_state_extend (IM (inl ieqv))
-                    (existT (fun n0 : nat => t (S n0) -> vstate (IM (inl ieqv))) n bs)
-                    sn)))
+              (state_update equivocator_IM s eqv
+                 (equivocator_state_extend (IM eqv)
+                    (existT (fun n0 : nat => t (S n0) -> vstate (IM eqv)) nieqv bsieqv) sieqv')))
               with (equivocators_state_project eqv_choice s)
-              ; try assumption.
+            ; [assumption|].
             apply functional_extensionality_dep.
-            intros [eqv'|neqv']; unfold equivocators_state_project.
-            --- destruct (eqv_choice eqv') eqn:Heqv'; try reflexivity.
-              destruct (decide (inl eqv' = inl ieqv)).
-              +++ inversion e. subst.
-                rewrite state_update_eq.
-                unfold equivocator_state_extend.
-                rewrite Hsieqv.
-                specialize (Heqvs ieqv).
-                rewrite Heqv' in Heqvs. simpl in Heqvs.
-                rewrite Hsieqv in Heqvs. simpl in Heqvs.
-                destruct (le_lt_dec (S n) n1). { lia. }
-                destruct (le_lt_dec (S (S n)) n1). { lia. }
-                rewrite to_nat_of_nat.
-                destruct (nat_eq_dec n1 (S n)). { lia. }
-                f_equal. apply of_nat_ext.
-              +++ rewrite state_update_neq; try assumption. reflexivity.
-            --- rewrite state_update_neq; try reflexivity.
-              intro contra. discriminate contra.
-      -- destruct Hv as [Hi Hv].
-        destruct (le_lt_dec (S (projT1 (s (inl ieqv)))) i). { lia. }
-        unfold fst in Ht.
-        destruct (vtransition (IM (inl ieqv)) li (projT2 (s (inl ieqv)) (of_nat_lt l), om0))
-          as (sieqv', om0') eqn:Ht'.
-        destruct fi eqn:Hfi; inversion Ht; subst si' om'; clear Ht.
-        ++ pose
-          (equivocators_choice_update
-            (fun eqv => NewMachine _ (proj1_sig (vs0 (IM (inl eqv)))))
-            ieqv (Existing _ i false)
-          ) as eqv_choice'.
-          specialize (IHHes1 eqv_choice') as Hs_om'.
-          spec Hs_om'.
-          { intro eqv'. unfold eqv_choice'.
-            destruct (decide (eqv' = ieqv)).
-            + subst. rewrite equivocators_choice_update_eq. assumption.
-            + rewrite equivocators_choice_update_neq; try assumption.
-              simpl. destruct (vs0 (IM (inl eqv'))). assumption.
-          }
-          destruct Hs_om' as [_oms Hs_om'].
-          destruct IHHes2 as [_som0 Hom0].
-          specialize (Hgen_om' _ _ Hs_om' _ _ Hom0).
-          spec Hgen_om'.
-          { split; try exact I.
-            unfold free_composite_valid.
-            unfold equivocators_state_project.
-            unfold eqv_choice'.
-            rewrite equivocators_choice_update_eq.
-            destruct (s (inl ieqv)) as (nieqv, bsieqv).
-            simpl in Hi.
-            destruct (le_lt_dec (S nieqv) i). { lia. }
-            replace (of_nat_lt l0) with (of_nat_lt Hi); try apply of_nat_ext.
-            assumption.
-          }
-          remember (equivocators_state_project eqv_choice' s) as sp.
-          simpl in Hgen_om'.
-          subst sp. unfold equivocators_state_project at 1 in Hgen_om'.
-          unfold eqv_choice' at 1 in Hgen_om'.
-          rewrite equivocators_choice_update_eq in Hgen_om'.
-          destruct (s (inl ieqv)) as (nieqv, bsieqv) eqn:Hsieqv.
+            intros eqv'. unfold equivocators_state_project.
+            destruct (eqv_choice eqv') eqn:Heqv'; [reflexivity|].
+            destruct (decide (eqv' = eqv))
+            ; [|rewrite state_update_neq; [reflexivity|assumption]].
+            subst.
+            rewrite state_update_eq.
+            unfold equivocator_state_extend.
+            rewrite Hsieqv.
+            specialize (Heqvs eqv).
+            rewrite Heqv' in Heqvs. simpl in Heqvs.
+            rewrite Hsieqv in Heqvs. simpl in Heqvs.
+            destruct (le_lt_dec (S nieqv) n0); [lia|].
+            destruct (le_lt_dec (S (S nieqv)) n0); [lia|].
+            rewrite to_nat_of_nat.
+            destruct (nat_eq_dec n0 (S nieqv)); [lia|].
+            f_equal. apply of_nat_ext.
+      ++ pose
+        (equivocators_choice_update
+          (fun eqv => NewMachine _ (proj1_sig (vs0 (IM (eqv)))))
+          eqv (Existing _ i false)
+        ) as eqv_choice'.
+        specialize (IHHes1 eqv_choice') as Hs_om'.
+        spec Hs_om'.
+        { intro eqv'. unfold eqv_choice'.
+          destruct (decide (eqv' = eqv)).
+          + subst. rewrite equivocators_choice_update_eq. assumption.
+          + rewrite equivocators_choice_update_neq by assumption.
+            simpl. destruct (vs0 (IM (eqv'))). assumption.
+        }
+        destruct Hs_om' as [_oms Hs_om'].
+        destruct IHHes2 as [_som0 Hom0].
+        specialize (Hgen_om' _ _ Hs_om' _ _ Hom0).
+        spec Hgen_om'.
+        { split; [|exact I].
+          unfold free_composite_valid.
+          unfold equivocators_state_project.
+          unfold eqv_choice'.
+          rewrite equivocators_choice_update_eq.
+          destruct (s eqv) as (nieqv, bsieqv).
           simpl in Hi.
-          destruct (le_lt_dec (S nieqv) i). { lia. }
-          simpl in l. simpl in Ht'.
-          replace (of_nat_lt l) with (of_nat_lt Hi) in * by apply of_nat_ext.
-          clear l.
-          replace (of_nat_lt l0) with (of_nat_lt Hi) in * by apply of_nat_ext.
-          clear l0.
-          rewrite Ht' in Hgen_om'.
-          split; try (eexists _; apply Hgen_om').
-          intros eqv_choice Heqv.
-          unfold_transition Hgen_om'.
-          destruct (eqv_choice ieqv) as [sieqv | iieqv fieqv] eqn:Hieqv.
-          ** assert (Heqvs : proper_equivocators_choice eqv_choice s).
-            { intro eqv'. specialize (Heqv eqv').
-              simpl in *.
-              destruct (decide (inl eqv' = inl ieqv))
-              ; try (rewrite state_update_neq in Heqv; assumption).
-              inversion e. subst. rewrite state_update_eq in Heqv.
-              rewrite Hieqv in *. simpl in Heqv. assumption.
-            }
-            specialize (IHHes1 _ Heqvs).
-            replace
-              (equivocators_state_project eqv_choice
-              (state_update equivocator_IM s (inl ieqv)
-                 (equivocator_state_extend (IM (inl ieqv))
-                    (existT (fun n : nat => t (S n) -> vstate (IM (inl ieqv))) nieqv bsieqv) sieqv')))
-              with (equivocators_state_project eqv_choice s)
-              ; try assumption.
-            apply functional_extensionality_dep.
-            intros [eqv'|neqv']; unfold equivocators_state_project.
-            --- destruct (eqv_choice eqv') eqn:Heqv'; try reflexivity.
-              destruct (decide (inl eqv' = inl ieqv)).
-              +++ inversion e. subst.
-                rewrite state_update_eq.
-                unfold equivocator_state_extend.
-                rewrite Hsieqv.
-                specialize (Heqvs ieqv).
-                rewrite Heqv' in Heqvs. simpl in Heqvs.
-                rewrite Hsieqv in Heqvs. simpl in Heqvs.
-                destruct (le_lt_dec (S nieqv) n). { lia. }
-                destruct (le_lt_dec (S (S nieqv)) n). { lia. }
-                rewrite to_nat_of_nat.
-                destruct (nat_eq_dec n (S nieqv)). { lia. }
-                f_equal. apply of_nat_ext.
-              +++ rewrite state_update_neq; try assumption. reflexivity.
-            --- rewrite state_update_neq; try reflexivity.
-              intro contra. discriminate contra.
-          ** specialize (Heqv ieqv) as Heqvi. unfold proper_descriptor in Heqvi.
-            rewrite Hieqv in Heqvi. rewrite state_update_eq in Heqvi.
-            simpl in Heqvi.
-            destruct (nat_eq_dec iieqv (S nieqv)).
-            --- subst.
-              pose (equivocators_choice_update eqv_choice ieqv (Existing _ i false)) as eqv_choice''.
-              specialize (IHHes1 eqv_choice'').
-              spec IHHes1.
-              { intro eqv'. spec Heqv eqv'.
-                destruct (decide (inl eqv' = inl ieqv)).
-                - inversion e. subst.
-                  unfold eqv_choice''.
-                  rewrite equivocators_choice_update_eq.
-                  simpl. rewrite Hsieqv.
-                  assumption.
-                - rewrite state_update_neq in Heqv; try assumption.
-                  unfold eqv_choice''.
-                  assert (n' : eqv' <> ieqv) by (intro contra; subst; elim n; reflexivity).
-                  rewrite equivocators_choice_update_neq; assumption.
-              }
-              specialize (Hgen (existT _ (inl ieqv) li)).
-              destruct IHHes1 as [_oms' Hs].
-              specialize (Hgen _ _ Hs _ _ Hom0).
-              spec Hgen.
-              { split; try exact I.
-                unfold free_composite_valid. unfold vvalid. simpl in Hv.
-                replace (equivocators_state_project eqv_choice'' s (inl ieqv)) with (bsieqv (of_nat_lt Hi)); try assumption.
+          destruct (le_lt_dec (S nieqv) i); [lia|].
+          replace (of_nat_lt l0) with (of_nat_lt Hi) by apply of_nat_ext.
+          assumption.
+        }
+        remember (equivocators_state_project eqv_choice' s) as sp.
+        simpl in Hgen_om'.
+        subst sp. unfold equivocators_state_project at 1 in Hgen_om'.
+        unfold eqv_choice' at 1 in Hgen_om'.
+        rewrite equivocators_choice_update_eq in Hgen_om'.
+        destruct (s eqv) as (nieqv, bsieqv) eqn:Hsieqv.
+        simpl in Hi.
+        destruct (le_lt_dec (S nieqv) i); [lia|].
+        simpl in Ht'.
+        replace (of_nat_lt l0) with (of_nat_lt Hi) in * by apply of_nat_ext.
+        clear l0.
+        simpl in l.
+        replace (of_nat_lt l) with (of_nat_lt Hi) in * by apply of_nat_ext.
+        rewrite Ht' in Hgen_om'.
+        split; [eexists _; apply Hgen_om'|].
+        intros eqv_choice Heqv.
+        destruct (eqv_choice eqv) as [sieqv | iieqv fieqv] eqn:Hieqv.
+        ** assert (Heqvs : proper_equivocators_choice eqv_choice s).
+          { intro eqv'. specialize (Heqv eqv').
+            simpl in *.
+            destruct (decide (eqv' = eqv))
+            ; [| rewrite state_update_neq in Heqv; assumption].
+            subst. rewrite state_update_eq in Heqv.
+            rewrite Hieqv in *. simpl in Heqv. assumption.
+          }
+          specialize (IHHes1 _ Heqvs).
+          replace
+            (equivocators_state_project eqv_choice
+            (state_update equivocator_IM s eqv
+               (equivocator_state_update (IM eqv)
+                  (existT (fun n : nat => t (S n) -> vstate (IM eqv)) nieqv bsieqv)
+                  (of_nat_lt l) sieqv')))
+            with (equivocators_state_project eqv_choice s)
+            ; [assumption|].
+          apply functional_extensionality_dep.
+          intros eqv'. unfold equivocators_state_project.
+          destruct (eqv_choice eqv') eqn:Heqv'; [reflexivity|].
+          destruct (decide (eqv' = eqv)).
+          +++ subst.
+            rewrite Hieqv in Heqv'. congruence.
+          +++ rewrite state_update_neq by assumption. reflexivity.
+        ** specialize (Heqv eqv) as Heqvi. unfold proper_descriptor in Heqvi.
+          rewrite Hieqv in Heqvi. rewrite state_update_eq in Heqvi.
+          simpl in Heqvi.
+          destruct (nat_eq_dec iieqv i).
+          --- subst.
+            pose (equivocators_choice_update eqv_choice eqv (Existing _ i false)) as eqv_choice''.
+            specialize (IHHes1 eqv_choice'').
+            spec IHHes1.
+            { intro eqv'. spec Heqv eqv'.
+              destruct (decide (eqv' = eqv)).
+              - subst.
                 unfold eqv_choice''.
-                unfold equivocators_state_project.
                 rewrite equivocators_choice_update_eq.
-                rewrite Hsieqv.
-                destruct (le_lt_dec (S nieqv) i). { lia. }
-                f_equal. apply of_nat_ext.
-              }
-              unfold transition in Hgen.
-              unfold X in Hgen at 2. unfold free_composite_vlsm in Hgen.
-              unfold composite_vlsm in Hgen.
-              unfold mk_vlsm in Hgen.
-              unfold machine in Hgen.
-              unfold projT2 in Hgen.
-              unfold composite_vlsm_machine in Hgen.
-              unfold composite_transition in Hgen.
-              unfold equivocators_state_project at 1 in Hgen.
-              unfold eqv_choice'' in Hgen.
-              rewrite equivocators_choice_update_eq in Hgen.
-              rewrite Hsieqv in Hgen.
-              destruct (le_lt_dec (S nieqv) i). { lia. }
-              replace (of_nat_lt l) with (of_nat_lt Hi) in * by apply of_nat_ext.
-              rewrite Ht' in Hgen.
-              exists om0'.
-              replace
-                (equivocators_state_project eqv_choice
-                (state_update equivocator_IM s (inl ieqv)
-                   (equivocator_state_extend (IM (inl ieqv))
-                      (existT (fun n : nat => t (S n) -> vstate (IM (inl ieqv))) nieqv bsieqv) sieqv')))
-                with (state_update IM
-                (equivocators_state_project
-                   (equivocators_choice_update eqv_choice ieqv (Existing (IM (inl ieqv)) i false)) s)
-                (inl ieqv) sieqv')
-                ; try assumption.
-              apply functional_extensionality_dep.
-              intro i'.
-              rewrite equivocators_state_project_state_update_eqv.
-              destruct (decide (i' = inl ieqv)).
-              +++ subst. repeat rewrite state_update_eq.
-                rewrite Hieqv. unfold equivocator_state_extend.
-                unfold projT1. unfold projT2.
-                destruct (le_lt_dec (S (S nieqv)) (S nieqv)). { lia. }
-                rewrite to_nat_of_nat.
-                destruct (nat_eq_dec (S nieqv) (S nieqv)); try (elim n; reflexivity).
-                reflexivity.
-              +++ repeat rewrite state_update_neq; try assumption.
-                unfold equivocators_state_project.
-                destruct i'; try reflexivity.
-                rewrite equivocators_choice_update_neq
-                ; try (intro contra; subst; elim n; reflexivity).
-                reflexivity.
-            --- assert (Heqvs : proper_equivocators_choice eqv_choice s).
-              { intro eqv'. specialize (Heqv eqv').
-                simpl in *.
-                destruct (decide (inl eqv' = inl ieqv))
-                ; try (rewrite state_update_neq in Heqv; assumption).
-                inversion e. subst. rewrite state_update_eq in Heqv.
-                rewrite Hieqv in *. simpl in Heqv. simpl.
-                rewrite Hsieqv. simpl. lia.
-              }
-              specialize (IHHes1 _ Heqvs).
-              replace
-                (equivocators_state_project eqv_choice
-                (state_update equivocator_IM s (inl ieqv)
-                   (equivocator_state_extend (IM (inl ieqv))
-                      (existT (fun n0 : nat => t (S n0) -> vstate (IM (inl ieqv))) nieqv bsieqv) sieqv')))
-                with (equivocators_state_project eqv_choice s)
-                ; try assumption.
-              apply functional_extensionality_dep.
-              intros [eqv'|neqv']; unfold equivocators_state_project.
-              +++ destruct (eqv_choice eqv') eqn:Heqv'; try reflexivity.
-                destruct (decide (inl eqv' = inl ieqv)).
-                *** inversion e. subst.
-                  rewrite state_update_eq.
-                  unfold equivocator_state_extend.
-                  rewrite Hsieqv.
-                  specialize (Heqvs ieqv).
-                  rewrite Heqv' in Heqvs. simpl in Heqvs.
-                  rewrite Hsieqv in Heqvs. simpl in Heqvs.
-                  destruct (le_lt_dec (S nieqv) n0). { lia. }
-                  destruct (le_lt_dec (S (S nieqv)) n0). { lia. }
-                  rewrite to_nat_of_nat.
-                  destruct (nat_eq_dec n0 (S nieqv)). { lia. }
-                  f_equal. apply of_nat_ext.
-                *** rewrite state_update_neq; try assumption. reflexivity.
-              +++ rewrite state_update_neq; try reflexivity.
-                intro contra. discriminate contra.
-        ++ pose
-          (equivocators_choice_update
-            (fun eqv => NewMachine _ (proj1_sig (vs0 (IM (inl eqv)))))
-            ieqv (Existing _ i false)
-          ) as eqv_choice'.
-          specialize (IHHes1 eqv_choice') as Hs_om'.
-          spec Hs_om'.
-          { intro eqv'. unfold eqv_choice'.
-            destruct (decide (eqv' = ieqv)).
-            + subst. rewrite equivocators_choice_update_eq. assumption.
-            + rewrite equivocators_choice_update_neq; try assumption.
-              simpl. destruct (vs0 (IM (inl eqv'))). assumption.
-          }
-          destruct Hs_om' as [_oms Hs_om'].
-          destruct IHHes2 as [_som0 Hom0].
-          specialize (Hgen_om' _ _ Hs_om' _ _ Hom0).
-          spec Hgen_om'.
-          { split; try exact I.
-            unfold free_composite_valid.
-            unfold equivocators_state_project.
-            unfold eqv_choice'.
-            rewrite equivocators_choice_update_eq.
-            destruct (s (inl ieqv)) as (nieqv, bsieqv).
-            simpl in Hi.
-            destruct (le_lt_dec (S nieqv) i). { lia. }
-            replace (of_nat_lt l0) with (of_nat_lt Hi); try apply of_nat_ext.
-            assumption.
-          }
-          remember (equivocators_state_project eqv_choice' s) as sp.
-          simpl in Hgen_om'.
-          subst sp. unfold equivocators_state_project at 1 in Hgen_om'.
-          unfold eqv_choice' at 1 in Hgen_om'.
-          rewrite equivocators_choice_update_eq in Hgen_om'.
-          destruct (s (inl ieqv)) as (nieqv, bsieqv) eqn:Hsieqv.
-          simpl in Hi.
-          destruct (le_lt_dec (S nieqv) i). { lia. }
-          simpl in Ht'.
-          replace (of_nat_lt l0) with (of_nat_lt Hi) in * by apply of_nat_ext.
-          clear l0.
-          simpl in l.
-          replace (of_nat_lt l) with (of_nat_lt Hi) in * by apply of_nat_ext.
-          rewrite Ht' in Hgen_om'.
-          split; try (eexists _; apply Hgen_om').
-          intros eqv_choice Heqv.
-          destruct (eqv_choice ieqv) as [sieqv | iieqv fieqv] eqn:Hieqv.
-          ** assert (Heqvs : proper_equivocators_choice eqv_choice s).
+                simpl. rewrite Hsieqv.
+                assumption.
+              - rewrite state_update_neq in Heqv by assumption.
+                unfold eqv_choice''.
+                rewrite equivocators_choice_update_neq; assumption.
+            }
+            specialize (Hgen (existT _ eqv li)).
+            destruct IHHes1 as [_oms' Hs].
+            specialize (Hgen _ _ Hs _ _ Hom0).
+            spec Hgen.
+            { split; [|exact I].
+              unfold free_composite_valid. unfold vvalid. simpl in Hv.
+              replace (equivocators_state_project eqv_choice'' s eqv) with (bsieqv (of_nat_lt Hi))
+              ; [assumption|].
+              unfold eqv_choice''.
+              unfold equivocators_state_project.
+              rewrite equivocators_choice_update_eq.
+              rewrite Hsieqv.
+              destruct (le_lt_dec (S nieqv) i); [lia|].
+              f_equal. apply of_nat_ext.
+            }
+            unfold transition in Hgen.
+            unfold X in Hgen at 2. unfold free_composite_vlsm in Hgen.
+            unfold composite_vlsm in Hgen.
+            unfold mk_vlsm in Hgen.
+            unfold machine in Hgen.
+            unfold projT2 in Hgen.
+            unfold composite_vlsm_machine in Hgen.
+            unfold composite_transition in Hgen.
+            unfold equivocators_state_project at 1 in Hgen.
+            unfold eqv_choice'' in Hgen.
+            rewrite equivocators_choice_update_eq in Hgen.
+            rewrite Hsieqv in Hgen.
+            destruct (le_lt_dec (S nieqv) i); [lia|].
+            replace (of_nat_lt l0) with (of_nat_lt Hi) in * by apply of_nat_ext.
+            rewrite Ht' in Hgen.
+            exists om0'.
+            replace
+              (equivocators_state_project eqv_choice
+              (state_update equivocator_IM s eqv
+                 (equivocator_state_update (IM eqv)
+                    (existT (fun n : nat => t (S n) -> vstate (IM eqv)) nieqv bsieqv)
+                    (of_nat_lt l) sieqv')))
+              with (state_update IM
+              (equivocators_state_project
+                 (equivocators_choice_update eqv_choice eqv (Existing (IM eqv) i false)) s)
+              eqv sieqv')
+            ; [assumption|].
+            apply functional_extensionality_dep.
+            intro i'.
+            rewrite equivocators_state_project_state_update_eqv.
+            destruct (decide (i' = eqv)).
+            +++ subst. repeat rewrite state_update_eq.
+              rewrite Hieqv. unfold equivocator_state_update at 1.
+              unfold projT1.
+              destruct (le_lt_dec (S nieqv) i); [lia|].
+              unfold equivocator_state_update. unfold projT2.
+              rewrite eq_dec_if_true by apply of_nat_ext.
+              reflexivity.
+            +++ repeat rewrite state_update_neq by assumption.
+              unfold equivocators_state_project.
+              rewrite equivocators_choice_update_neq by assumption.
+              reflexivity.
+          --- assert (Heqvs : proper_equivocators_choice eqv_choice s).
             { intro eqv'. specialize (Heqv eqv').
               simpl in *.
-              destruct (decide (inl eqv' = inl ieqv))
-              ; try (rewrite state_update_neq in Heqv; assumption).
-              inversion e. subst. rewrite state_update_eq in Heqv.
-              rewrite Hieqv in *. simpl in Heqv. assumption.
+              destruct (decide (eqv' = eqv))
+              ; [|rewrite state_update_neq in Heqv; assumption].
+              subst. rewrite state_update_eq in Heqv.
+              rewrite Hieqv in *. simpl in Heqv. simpl.
+              rewrite Hsieqv. simpl. lia.
             }
             specialize (IHHes1 _ Heqvs).
             replace
               (equivocators_state_project eqv_choice
-              (state_update equivocator_IM s (inl ieqv)
-                 (equivocator_state_update (IM (inl ieqv))
-                    (existT (fun n : nat => t (S n) -> vstate (IM (inl ieqv))) nieqv bsieqv)
+              (state_update equivocator_IM s eqv
+                 (equivocator_state_update (IM eqv)
+                    (existT (fun n0 : nat => t (S n0) -> vstate (IM eqv)) nieqv bsieqv)
                     (of_nat_lt l) sieqv')))
               with (equivocators_state_project eqv_choice s)
-              ; try assumption.
+            ; [assumption|].
             apply functional_extensionality_dep.
-            intros [eqv'|neqv']; unfold equivocators_state_project.
-            --- destruct (eqv_choice eqv') eqn:Heqv'; try reflexivity.
-              destruct (decide (inl eqv' = inl ieqv)).
-              +++ inversion e. subst.
-                rewrite Hieqv in Heqv'. discriminate Heqv'.
-              +++ rewrite state_update_neq; try assumption. reflexivity.
-            --- rewrite state_update_neq; try reflexivity.
-              intro contra. discriminate contra.
-          ** specialize (Heqv ieqv) as Heqvi. unfold proper_descriptor in Heqvi.
-            rewrite Hieqv in Heqvi. rewrite state_update_eq in Heqvi.
-            simpl in Heqvi.
-            destruct (nat_eq_dec iieqv i).
-            --- subst.
-              pose (equivocators_choice_update eqv_choice ieqv (Existing _ i false)) as eqv_choice''.
-              specialize (IHHes1 eqv_choice'').
-              spec IHHes1.
-              { intro eqv'. spec Heqv eqv'.
-                destruct (decide (inl eqv' = inl ieqv)).
-                - inversion e. subst.
-                  unfold eqv_choice''.
-                  rewrite equivocators_choice_update_eq.
-                  simpl. rewrite Hsieqv.
-                  assumption.
-                - rewrite state_update_neq in Heqv; try assumption.
-                  unfold eqv_choice''.
-                  assert (n' : eqv' <> ieqv) by (intro contra; subst; elim n; reflexivity).
-                  rewrite equivocators_choice_update_neq; assumption.
-              }
-              specialize (Hgen (existT _ (inl ieqv) li)).
-              destruct IHHes1 as [_oms' Hs].
-              specialize (Hgen _ _ Hs _ _ Hom0).
-              spec Hgen.
-              { split; try exact I.
-                unfold free_composite_valid. unfold vvalid. simpl in Hv.
-                replace (equivocators_state_project eqv_choice'' s (inl ieqv)) with (bsieqv (of_nat_lt Hi)); try assumption.
-                unfold eqv_choice''.
-                unfold equivocators_state_project.
-                rewrite equivocators_choice_update_eq.
-                rewrite Hsieqv.
-                destruct (le_lt_dec (S nieqv) i). { lia. }
-                f_equal. apply of_nat_ext.
-              }
-              unfold transition in Hgen.
-              unfold X in Hgen at 2. unfold free_composite_vlsm in Hgen.
-              unfold composite_vlsm in Hgen.
-              unfold mk_vlsm in Hgen.
-              unfold machine in Hgen.
-              unfold projT2 in Hgen.
-              unfold composite_vlsm_machine in Hgen.
-              unfold composite_transition in Hgen.
-              unfold equivocators_state_project at 1 in Hgen.
-              unfold eqv_choice'' in Hgen.
-              rewrite equivocators_choice_update_eq in Hgen.
-              rewrite Hsieqv in Hgen.
-              destruct (le_lt_dec (S nieqv) i). { lia. }
-              replace (of_nat_lt l0) with (of_nat_lt Hi) in * by apply of_nat_ext.
-              rewrite Ht' in Hgen.
-              exists om0'.
-              replace
-                (equivocators_state_project eqv_choice
-                (state_update equivocator_IM s (inl ieqv)
-                   (equivocator_state_update (IM (inl ieqv))
-                      (existT (fun n : nat => t (S n) -> vstate (IM (inl ieqv))) nieqv bsieqv)
-                      (of_nat_lt l) sieqv')))
-                with (state_update IM
-                (equivocators_state_project
-                   (equivocators_choice_update eqv_choice ieqv (Existing (IM (inl ieqv)) i false)) s)
-                (inl ieqv) sieqv')
-                ; try assumption.
-              apply functional_extensionality_dep.
-              intro i'.
-              rewrite equivocators_state_project_state_update_eqv.
-              destruct (decide (i' = inl ieqv)).
-              +++ subst. repeat rewrite state_update_eq.
-                rewrite Hieqv. unfold equivocator_state_update at 1.
-                unfold projT1.
-                destruct (le_lt_dec (S nieqv) i). { lia. }
-                unfold equivocator_state_update. unfold projT2.
-                rewrite eq_dec_if_true; try reflexivity.
-                apply of_nat_ext.
-              +++ repeat rewrite state_update_neq; try assumption.
-                unfold equivocators_state_project.
-                destruct i'; try reflexivity.
-                rewrite equivocators_choice_update_neq
-                ; try (intro contra; subst; elim n; reflexivity).
-                reflexivity.
-            --- assert (Heqvs : proper_equivocators_choice eqv_choice s).
-              { intro eqv'. specialize (Heqv eqv').
-                simpl in *.
-                destruct (decide (inl eqv' = inl ieqv))
-                ; try (rewrite state_update_neq in Heqv; assumption).
-                inversion e. subst. rewrite state_update_eq in Heqv.
-                rewrite Hieqv in *. simpl in Heqv. simpl.
-                rewrite Hsieqv. simpl. lia.
-              }
-              specialize (IHHes1 _ Heqvs).
-              replace
-                (equivocators_state_project eqv_choice
-                (state_update equivocator_IM s (inl ieqv)
-                   (equivocator_state_update (IM (inl ieqv))
-                      (existT (fun n0 : nat => t (S n0) -> vstate (IM (inl ieqv))) nieqv bsieqv)
-                      (of_nat_lt l) sieqv')))
-                with (equivocators_state_project eqv_choice s)
-                ; try assumption.
-              apply functional_extensionality_dep.
-              intros [eqv'|neqv']; unfold equivocators_state_project.
-              +++ destruct (eqv_choice eqv') eqn:Heqv'; try reflexivity.
-                destruct (decide (inl eqv' = inl ieqv)).
-                *** inversion e. subst.
-                  rewrite state_update_eq.
-                  unfold equivocator_state_extend.
-                  rewrite Hsieqv.
-                  specialize (Heqvs ieqv).
-                  rewrite Heqv' in Heqvs. simpl in Heqvs.
-                  rewrite Hsieqv in Heqvs. simpl in Heqvs.
-                  destruct (le_lt_dec (S nieqv) n0). { lia. }
-                  destruct (le_lt_dec (S (S nieqv)) n0). { lia. }
-                  unfold equivocator_state_update.
-                  unfold projT1.
-                  destruct (le_lt_dec (S nieqv) n0). { lia. }
-                  rewrite Hieqv in Heqv'.
-                  inversion Heqv'. subst n0 b. clear Heqv'.
-                  unfold projT2.
-                  rewrite eq_dec_if_false; try (f_equal; apply of_nat_ext).
-                  intro contra. elim n.
-                  apply (f_equal to_nat) in contra.
-                  repeat rewrite to_nat_of_nat in contra.
-                  inversion contra. reflexivity.
-                *** rewrite state_update_neq; try assumption. reflexivity.
-              +++ rewrite state_update_neq; try reflexivity.
-                intro contra. discriminate contra.
-    * specialize (Hgen (existT _ (inr ineqv) li)).
-      unfold vvalid in Hv. simpl in Hv.
-      unfold vtransition in Ht. simpl in Ht.
-      pose (fun eqv => NewMachine _ (proj1_sig (vs0 (IM (inl eqv))))) as eqv_choice.
-      specialize (IHHes1 eqv_choice) as Hs_om'.
-      spec Hs_om'.
-      { intro eqv'. unfold eqv_choice.
-        simpl. destruct (vs0 (IM (inl eqv'))). assumption.
-      }
-      destruct Hs_om' as [_oms Hs_om'].
-      destruct IHHes2 as [_som0 Hom0].
-      specialize (Hgen _ _ Hs_om' _ _ Hom0) as Hgen_om'.
-      spec Hgen_om'. { split; try exact I. assumption. }
-      remember (equivocators_state_project eqv_choice s) as sp.
-      simpl in Hgen_om'.
-      unfold vtransition in Hgen_om'.
-      subst sp. unfold equivocators_state_project at 1 in Hgen_om'.
-      rewrite Ht in Hgen_om'.
-      split; try (eexists _; apply Hgen_om').
-      clear eqv_choice Hgen_om' Hs_om'.
-      intros eqv_choice Heqv.
-      assert (Heqvs : proper_equivocators_choice eqv_choice s).
-      { intro eqv'. specialize (Heqv eqv').
-        rewrite state_update_neq in Heqv; congruence.
-      }
-      specialize (IHHes1 _ Heqvs).
-      destruct IHHes1 as [_oms' Hs].
-      specialize (Hgen _ _ Hs _ _ Hom0).
-      spec Hgen. { split; try exact I. assumption. }
-      unfold transition in Hgen.
-      unfold X in Hgen at 2. unfold free_composite_vlsm in Hgen.
-      unfold composite_vlsm in Hgen.
-      unfold mk_vlsm in Hgen.
-      unfold machine in Hgen.
-      unfold projT2 in Hgen.
-      unfold composite_vlsm_machine in Hgen.
-      unfold composite_transition in Hgen.
-      unfold equivocators_state_project at 1 in Hgen.
-      unfold vtransition in Hgen. rewrite Ht in Hgen.
-      exists om'.
-      rewrite equivocators_state_project_state_update_neqv.
-      assumption.
+            intros eqv'. unfold equivocators_state_project.
+            +++ destruct (eqv_choice eqv') eqn:Heqv'; [reflexivity|].
+              destruct (decide (eqv' = eqv))
+              ; [|rewrite state_update_neq; [reflexivity| assumption]].
+              subst.
+              rewrite state_update_eq.
+              unfold equivocator_state_extend.
+              rewrite Hsieqv.
+              specialize (Heqvs eqv).
+              rewrite Heqv' in Heqvs. simpl in Heqvs.
+              rewrite Hsieqv in Heqvs. simpl in Heqvs.
+              destruct (le_lt_dec (S nieqv) n0); [lia|].
+              destruct (le_lt_dec (S (S nieqv)) n0); [lia|].
+              unfold equivocator_state_update.
+              unfold projT1.
+              destruct (le_lt_dec (S nieqv) n0); [lia|].
+              rewrite Hieqv in Heqv'.
+              inversion Heqv'. subst n0 b. clear Heqv'.
+              unfold projT2.
+              rewrite eq_dec_if_false; [f_equal; apply of_nat_ext|].
+              intro contra. elim n.
+              apply (f_equal to_nat) in contra.
+              repeat rewrite to_nat_of_nat in contra.
+              inversion contra. reflexivity.
 Qed.
 
 End fully_equivocating_composition.
