VLSM/Equivocators/Composition/Projections.v
@@ -1,0 +1,847 @@
+Require Import
+  List Coq.Vectors.Fin FinFun
+  Arith.Compare_dec Lia
+  Program
+  Coq.Logic.JMeq
+  .
+Import ListNotations.
+From CasperCBC
+  Require Import
+    Preamble ListExtras FinExtras
+    VLSM.Common VLSM.Composition VLSM.Equivocation
+    VLSM.Equivocators.Common VLSM.Equivocators.Projections
+    VLSM.Equivocators.MessageProperties
+    VLSM.Equivocators.Composition.Common
+    .
+
+Section equivocators_composition_projections.
+
+Context {message : Type}
+  {equiv_index : Type}
+  (index := equiv_index)
+  {IndEqDec : EqDecision index}
+  (IM : index -> VLSM message)
+  (Hbs : forall i : index, has_been_sent_capability (IM i))
+  (i0 : index)
+  (X := free_composite_vlsm IM i0)
+  (index_listing : list index)
+  (finite_index : Listing index_listing)
+  (equivocators_choice := equivocators_choice IM)
+  (equivocators_no_equivocations_vlsm := equivocators_no_equivocations_vlsm IM Hbs i0 index_listing finite_index)
+  (equivocators_state_project := equivocators_state_project IM i0)
+  (equivocator_IM := equivocator_IM IM)
+  (equivocators_choice_update := equivocators_choice_update IM)
+  (proper_equivocators_choice := proper_equivocators_choice IM i0)
+  .
+
+Definition equivocators_transition_item_project
+  (eqv_choice : equivocators_choice)
+  (item : vtransition_item equivocators_no_equivocations_vlsm)
+  : option (option (vtransition_item X) * equivocators_choice)
+  :=
+  match item with {| l := el; input := iom; output := oom; destination := s |} =>
+    let sx := equivocators_state_project eqv_choice s in
+    let (eqv, li) := el in
+    let deqv := eqv_choice eqv in
+    match
+      equivocator_vlsm_transition_item_project
+        (IM eqv)
+        {| l := li; input := iom; output := oom; destination := s eqv |}
+        deqv
+        with
+    | Some (Some item', deqv') =>
+      Some
+        (Some (@Build_transition_item message (@type message X)
+          (existT (fun n : index => vlabel (IM n)) eqv (l item'))
+          iom sx oom)
+        , equivocators_choice_update eqv_choice eqv deqv')
+    | Some (None, deqv') => Some (None, equivocators_choice_update eqv_choice eqv deqv')
+    | None => None
+    end
+  end.
+
+Lemma equivocators_transition_item_project_proper
+  (eqv_choice : equivocators_choice)
+  (item : vtransition_item equivocators_no_equivocations_vlsm)
+  (Hproper : proper_equivocators_choice eqv_choice (destination item))
+  : equivocators_transition_item_project eqv_choice item <> None.
+Proof.
+  destruct item. simpl.
+  destruct l as [e v].
+  intro contra.
+  spec Hproper e. simpl in Hproper.
+  elim
+    (equivocator_transition_item_project_proper (IM e)
+      (@Build_transition_item message (@equivocator_type message (IM e))
+        v input (destination e) output)
+      (eqv_choice e) Hproper).
+  simpl in contra. simpl.
+  destruct
+    (equivocator_vlsm_transition_item_project (IM e)
+      (@Build_transition_item message (@equivocator_type message (IM e))
+        v input (destination e) output)
+      (eqv_choice e))
+  ; [|reflexivity].
+  destruct p. destruct o; congruence.
+Qed.
+
+Definition equivocators_trace_project_folder
+  (item : vtransition_item equivocators_no_equivocations_vlsm)
+  (result: option (list (vtransition_item X) * equivocators_choice))
+  : option (list (vtransition_item X) * equivocators_choice)
+  :=
+  match result with
+  | None => None
+  | Some (r, idescriptor) =>
+    match equivocators_transition_item_project idescriptor item with
+    | None => None
+    | Some (None, odescriptor) => Some (r, odescriptor)
+    | Some (Some item', odescriptor) => Some (item' :: r, odescriptor)
+    end
+  end.
+
+Lemma equivocators_trace_project_fold_None
+  (tr : list (vtransition_item equivocators_no_equivocations_vlsm))
+  : fold_right equivocators_trace_project_folder None tr = None.
+Proof.
+  induction tr; [reflexivity|]. simpl. rewrite IHtr. reflexivity.
+Qed.
+
+Lemma equivocators_trace_project_folder_additive
+  (tr : list (vtransition_item equivocators_no_equivocations_vlsm))
+  (itrX trX : list (vtransition_item X))
+  (ieqv_choice eqv_choice : equivocators_choice)
+  (Htr : fold_right equivocators_trace_project_folder (Some ([], ieqv_choice)) tr
+    = Some (trX, eqv_choice))
+  : fold_right equivocators_trace_project_folder (Some (itrX, ieqv_choice)) tr
+    = Some (trX ++ itrX, eqv_choice).
+Proof.
+  generalize dependent trX. revert eqv_choice ieqv_choice.
+  induction tr; intros.
+  - simpl in Htr. inversion Htr. reflexivity.
+  - simpl in Htr.
+    simpl.
+    destruct
+      (fold_right equivocators_trace_project_folder (Some ([], ieqv_choice)) tr)
+      as [(trX', eqv_choice')|] eqn:Hfld; [|discriminate Htr].
+    simpl in Htr.
+    destruct (equivocators_transition_item_project eqv_choice' a)
+      as [(oitem, eqv_choice'')|] eqn:Ha; [|congruence].
+    destruct oitem as [item'|]; inversion Htr; subst
+    ; specialize (IHtr _ _ _ Hfld)
+    ; rewrite IHtr
+    ; simpl
+    ; rewrite Ha
+    ; reflexivity.
+Qed.
+
+(**
+The projection of an [equivocators] trace is obtained by traversing the
+trace from right to left guided by the descriptors produced by
+[equivocators_transition_item_project] and gathering all non-empty
+[transition_item]s it produces.
+*)
+Definition equivocators_trace_project
+  (eqv_choice : equivocators_choice)
+  (tr : list (vtransition_item equivocators_no_equivocations_vlsm))
+  : option (list (vtransition_item X) * equivocators_choice)
+  :=
+  fold_right
+    equivocators_trace_project_folder
+    (Some ([], eqv_choice))
+    tr.
+
+Local Tactic Notation "unfold_transition"  hyp(Ht) :=
+  ( unfold transition in Ht; unfold equivocator_IM in Ht;
+  unfold equivocator_vlsm in Ht; unfold mk_vlsm in Ht;
+  unfold machine in Ht; unfold projT2 in Ht;
+  unfold equivocator_vlsm_machine in Ht; unfold equivocator_transition in Ht). 
+
+Lemma equivocators_protocol_trace_project
+  (final_choice : equivocators_choice)
+  (is : vstate equivocators_no_equivocations_vlsm)
+  (tr : list (vtransition_item equivocators_no_equivocations_vlsm))
+  (final_state := last (map destination tr) is)
+  (Hproper : proper_equivocators_choice final_choice final_state)
+  (Htr : finite_protocol_trace_from equivocators_no_equivocations_vlsm is tr)
+  : exists
+    (trX : list (vtransition_item X))
+    (initial_choice : equivocators_choice)
+    (isX := equivocators_state_project initial_choice is)
+    (Hproject: equivocators_trace_project final_choice tr = Some (trX, initial_choice))
+    (final_stateX := last (map destination trX) isX)
+    (Hfinal : equivocators_state_project final_choice final_state = final_stateX)
+    (Hproper : proper_equivocators_choice initial_choice is),
+    finite_protocol_trace_from X isX trX.
+Proof.
+  generalize dependent final_choice.
+  generalize dependent is.
+  induction tr; intros.
+  - exists []. simpl. exists final_choice.
+    exists eq_refl. exists eq_refl. exists Hproper.
+    constructor.
+    inversion Htr. subst. destruct H as [_om His].
+    apply (proj2 (equivocators_protocol_state_project IM Hbs i0 _ _ _ _ His) final_choice Hproper).
+  - unfold equivocators_trace_project. simpl.
+    inversion Htr. subst s' tl.
+    specialize (IHtr _ H2).
+    unfold final_state in Hproper.
+    rewrite map_cons in Hproper.
+    rewrite unroll_last in Hproper.
+    rewrite <- H in Hproper. simpl in Hproper.
+    specialize (IHtr _ Hproper).
+    destruct IHtr as [trX' [initial_choice' [Hproject [Hfinal [Hproper' HtrX']]]]].
+    unfold equivocators_trace_project in Hproject.
+    rewrite Hproject.
+    unfold equivocators_trace_project_folder.
+    destruct H3 as [[His [Hiom [Hv _]]] Ht].
+    simpl in Hv. simpl in Ht.
+    destruct l as (eqv, li).
+    destruct (vtransition (Common.equivocator_IM IM eqv) li (is eqv, iom)) as (si', om')
+      eqn:Ht'.
+    inversion Ht. subst s oom. clear Ht.
+    unfold final_state. rewrite map_cons. rewrite unroll_last. subst a.
+    clear final_state.
+    destruct His as [_omis His]. apply equivocators_protocol_state_project in His. destruct His as [_ His].
+    destruct Hiom as [_siom Hiom]. apply equivocators_protocol_state_project in Hiom.
+    destruct Hiom as [Hiom _].
+    simpl in *.
+    destruct (initial_choice' eqv) as [seqv | ieqv feqv] eqn:Heqv.
+    * eexists _. eexists _. exists eq_refl.
+      repeat split.
+      -- replace
+          (equivocators_state_project
+          (equivocators_choice_update initial_choice' eqv
+             (NewMachine (IM (eqv)) seqv)) is)
+          with
+            (equivocators_state_project initial_choice'
+            (state_update (Common.equivocator_IM IM) is (eqv) si'))
+          ;[assumption|].
+        assert
+          (Hinitial_choice' : equivocators_choice_update initial_choice' eqv
+          (NewMachine (IM (eqv)) seqv) = initial_choice').
+        { apply functional_extensionality_dep_good.
+          intro eqv'.  unfold equivocators_choice_update.
+          destruct (decide (eqv' = eqv)).
+          - subst eqv'.
+            rewrite equivocators_choice_update_eq. symmetry. assumption.
+          - rewrite equivocators_choice_update_neq by assumption. reflexivity.
+        }
+        rewrite Hinitial_choice'.
+        unfold equivocators_state_project.
+        rewrite equivocators_state_project_state_update_eqv.
+        rewrite Heqv.
+        apply functional_extensionality_dep_good.
+        intros eqv'.
+        destruct (decide (eqv = eqv')).
+        ** subst eqv'. rewrite state_update_eq. simpl.
+          unfold Common.equivocators_state_project.
+          rewrite Heqv. reflexivity.
+        ** rewrite state_update_neq; congruence.
+      -- intro eqv'.
+        destruct (decide (eqv' = eqv)).
+        ++ subst. unfold equivocators_choice_update. rewrite equivocators_choice_update_eq.
+          spec Hproper' eqv. rewrite Heqv in Hproper'. assumption.
+        ++ unfold equivocators_choice_update.
+          rewrite equivocators_choice_update_neq by assumption.
+          spec Hproper' eqv'.
+          rewrite state_update_neq in Hproper'; [assumption|]. congruence.
+      -- replace
+          (equivocators_state_project
+          (equivocators_choice_update initial_choice' eqv
+             (NewMachine (IM (eqv)) seqv)) is)
+          with
+            (equivocators_state_project initial_choice'
+            (state_update (Common.equivocator_IM IM) is (eqv) si'))
+        ; [assumption|].
+        rewrite (equivocators_state_project_state_update_eqv IM i0).
+        apply functional_extensionality_dep_good.
+        intro i'. destruct (decide (i' = (eqv))).
+        ++ subst. rewrite state_update_eq. rewrite Heqv.
+          unfold equivocators_state_project.
+          unfold Common.equivocators_state_project.
+          unfold equivocators_choice_update.
+          rewrite equivocators_choice_update_eq. reflexivity.
+        ++ rewrite state_update_neq by assumption.
+          unfold equivocators_state_project.
+          unfold Common.equivocators_state_project.
+          unfold equivocators_choice_update.
+          rewrite equivocators_choice_update_neq; congruence.
+    * rewrite state_update_eq.
+      destruct li as (li, di).
+      destruct si' as (nsi', bsi').
+      specialize (Hproper' eqv) as Hproper_eqv.
+      rewrite state_update_eq in Hproper_eqv.
+      rewrite Heqv in Hproper_eqv.
+      simpl in Hproper_eqv.
+      unfold equivocator_vlsm_transition_item_project.
+      destruct (le_lt_dec (S nsi') ieqv); [lia|].
+      unfold vvalid in Hv. simpl in Hv.
+      unfold vtransition in Ht'. 
+      unfold transition in Ht'. unfold Common.equivocator_IM in Ht'.
+      unfold equivocator_vlsm in Ht'. unfold mk_vlsm in Ht'.
+      unfold machine in Ht'. unfold projT2 in Ht'.
+      unfold equivocator_vlsm_machine in Ht'.
+      unfold equivocator_transition in Ht'.
+      unfold snd in Ht'.
+      destruct di as [sdi|idi fdi].
+      -- destruct Hv as [Hsdi _Hiom]. subst iom.
+        inversion Ht'. subst om'. clear Ht'.
+        unfold equivocator_state_extend in H0.
+        destruct (is (eqv)) as (is_eqv_n, is_eqv_s) eqn:His_eqv.
+        inversion H0. subst nsi'.
+        simpl_existT.
+        destruct (nat_eq_dec (S is_eqv_n) (S is_eqv_n)); [|lia].
+        destruct (nat_eq_dec (S ieqv) (S (S is_eqv_n))).
+        ++ inversion e0. subst ieqv. clear e e0.
+          eexists _. eexists _. exists eq_refl.
+          assert
+            (Hfinal' :
+            equivocators_state_project final_choice
+            (last (map destination tr)
+               (state_update (Common.equivocator_IM IM) is (eqv)
+                  (equivocator_state_extend (IM (eqv)) (existT (fun n : nat => t (S n) -> vstate (IM (eqv)))
+                  is_eqv_n is_eqv_s) sdi))) =
+            last (map destination trX')
+              (equivocators_state_project
+                 (equivocators_choice_update initial_choice' eqv
+                    (NewMachine (IM (eqv)) sdi)) is)
+            ).
+          { subst bsi'. simpl in *. rewrite Hfinal.
+            rewrite (equivocators_state_project_state_update_eqv IM i0).
+            rewrite Heqv.
+            unfold projT1. unfold projT2.
+            destruct (le_lt_dec (S (S is_eqv_n)) (S is_eqv_n)); [lia|].
+            f_equal.
+            apply functional_extensionality_dep_good.
+            rewrite to_nat_of_nat.
+            destruct (nat_eq_dec (S is_eqv_n) (S is_eqv_n)); [|lia].
+            intro i'. destruct (decide (i' = (eqv))).
+            - subst. rewrite state_update_eq.
+              unfold equivocators_state_project.
+              unfold Common.equivocators_state_project.
+              unfold equivocators_choice_update.
+              rewrite equivocators_choice_update_eq.
+              reflexivity.
+            - rewrite state_update_neq by assumption.
+              unfold equivocators_state_project.
+              unfold Common.equivocators_state_project.
+              unfold equivocators_choice_update.
+              rewrite equivocators_choice_update_neq; congruence.
+          }
+          exists Hfinal'.
+          assert
+            (Hproper'' :
+              proper_equivocators_choice
+                (equivocators_choice_update initial_choice' eqv
+                  (NewMachine (IM (eqv)) sdi)) is).
+          {
+          intro eqv'. spec Hproper' eqv'.  unfold equivocators_choice_update.
+          destruct (decide (eqv' = eqv)).
+          - subst. rewrite equivocators_choice_update_eq. assumption.
+          - rewrite equivocators_choice_update_neq by assumption.
+            rewrite state_update_neq in Hproper'; congruence.
+          }
+          exists Hproper''.
+          replace
+            (equivocators_state_project
+            (equivocators_choice_update initial_choice' eqv
+               (NewMachine (IM (eqv)) sdi)) is)
+            with
+              (equivocators_state_project initial_choice'
+              (state_update (Common.equivocator_IM IM) is
+                 (eqv)
+                 (existT (fun n : nat => t (S n) -> vstate (IM (eqv)))
+                  (S is_eqv_n) bsi')))
+          ; [assumption|].
+          subst bsi'.
+          unfold equivocators_state_project.
+          rewrite equivocators_state_project_state_update_eqv.
+          rewrite Heqv. unfold projT1. unfold projT2.
+          destruct (le_lt_dec (S (S is_eqv_n)) (S is_eqv_n)); [lia |].
+          rewrite to_nat_of_nat.
+          destruct ( nat_eq_dec (S is_eqv_n) (S is_eqv_n) ); [|congruence].
+          replace (of_nat_lt l0) with (of_nat_lt Hproper_eqv) in * by apply of_nat_ext.
+          clear l0.
+          replace (of_nat_lt l) with (of_nat_lt Hproper_eqv) in * by apply of_nat_ext.
+          clear l.
+          apply functional_extensionality_dep_good.
+          intro i.
+          unfold Common.equivocators_state_project at 2.
+          unfold equivocators_choice_update.
+          destruct (decide (i = (eqv))).
+          ** subst. rewrite state_update_eq.
+            rewrite equivocators_choice_update_eq.
+            reflexivity.
+          ** repeat rewrite state_update_neq by assumption.
+            unfold Common.equivocators_state_project.
+            rewrite equivocators_choice_update_neq; congruence.
+        ++ eexists _. eexists _. exists eq_refl.
+          assert
+            (Hfinal' :
+              equivocators_state_project final_choice
+                (last (map destination tr)
+                   (state_update (Common.equivocator_IM IM) is
+                      (eqv)
+                      (equivocator_state_extend (IM (eqv))
+                         (existT (fun n0 : nat => t (S n0) -> vstate (IM (eqv)))
+                            is_eqv_n is_eqv_s) sdi))) =
+              last (map destination trX')
+                (equivocators_state_project
+                   (equivocators_choice_update initial_choice' eqv
+                      (Existing (IM (eqv)) ieqv false)) is)
+            ).
+          { subst bsi'. simpl in *. rewrite Hfinal.
+            rewrite (equivocators_state_project_state_update_eqv IM i0).
+            rewrite Heqv.
+            unfold projT1. unfold projT2.
+            destruct (le_lt_dec (S (S is_eqv_n)) ieqv); [lia|].
+            f_equal.
+            apply functional_extensionality_dep_good.
+            rewrite to_nat_of_nat.
+            destruct (nat_eq_dec ieqv (S is_eqv_n)); [lia|].
+            intro i'. destruct (decide (i' = (eqv))).
+            - subst. rewrite state_update_eq.
+              unfold equivocators_state_project.
+              unfold Common.equivocators_state_project.
+              unfold equivocators_choice_update.
+              rewrite equivocators_choice_update_eq.
+              rewrite His_eqv.
+              destruct (le_lt_dec (S is_eqv_n) ieqv); [lia|].
+              f_equal. apply of_nat_ext.
+            - rewrite state_update_neq by assumption.
+              unfold equivocators_state_project.
+              unfold Common.equivocators_state_project.
+              unfold equivocators_choice_update.
+              rewrite equivocators_choice_update_neq; congruence.
+          }
+          exists Hfinal'.
+          assert
+            (Hproper'' :
+            proper_equivocators_choice
+            (equivocators_choice_update initial_choice' eqv
+               (Existing (IM (eqv)) ieqv false)) is).
+          {
+          intro eqv'. spec Hproper' eqv'.  unfold equivocators_choice_update.
+          destruct (decide (eqv' = eqv)).
+          - subst. rewrite equivocators_choice_update_eq.
+            simpl. rewrite His_eqv. simpl. lia.
+          - rewrite equivocators_choice_update_neq by assumption.
+            rewrite state_update_neq in Hproper'; congruence.
+          }
+          exists Hproper''.
+          replace
+            ((equivocators_state_project
+            (equivocators_choice_update initial_choice' eqv
+               (Existing (IM (eqv)) ieqv false)) is))
+            with
+              (equivocators_state_project initial_choice'
+              (state_update (Common.equivocator_IM IM) is
+                 (eqv)
+                 (existT (fun n : nat => t (S n) -> vstate (IM (eqv)))
+                  (S is_eqv_n) bsi')))
+          ; [assumption|].
+          unfold equivocators_state_project.
+          rewrite equivocators_state_project_state_update_eqv.
+          rewrite Heqv. unfold projT1. unfold projT2.
+          destruct (le_lt_dec (S (S is_eqv_n)) ieqv); [lia |].
+          replace (of_nat_lt l0) with (of_nat_lt Hproper_eqv) in * by apply of_nat_ext.
+          clear l0.
+          replace (of_nat_lt l) with (of_nat_lt Hproper_eqv) in * by apply of_nat_ext.
+          clear l.
+          apply functional_extensionality_dep_good.
+          intro i.
+          destruct (decide (i = (eqv))).
+          --- subst. rewrite state_update_eq.
+            unfold Common.equivocators_state_project.
+            unfold equivocators_choice_update.
+            rewrite equivocators_choice_update_eq.
+            rewrite to_nat_of_nat. rewrite His_eqv.
+            destruct (le_lt_dec (S is_eqv_n) ieqv); [lia|].
+            destruct (nat_eq_dec ieqv (S is_eqv_n)); [congruence|].
+            f_equal. apply of_nat_ext.
+          --- rewrite state_update_neq by assumption.
+            unfold Common.equivocators_state_project.
+            unfold equivocators_choice_update.
+            rewrite equivocators_choice_update_neq; congruence.
+    -- destruct Hv as [Hidi Hv].
+      destruct (le_lt_dec (S (projT1 (is (eqv)))) idi); [lia|].
+      replace (of_nat_lt l0) with (of_nat_lt Hidi) in * by apply of_nat_ext.
+      clear l0.
+      unfold fst in Ht'.
+      destruct (is (eqv)) as (neqv, bseqv) eqn:Hiseqv.
+      unfold projT2 in Ht'.
+      destruct (vtransition (IM (eqv)) li (bseqv (of_nat_lt Hidi), iom))
+        as (si', siom') eqn:Ht''.
+      destruct fdi.
+      ++ inversion Ht'. subst.
+        simpl_existT.
+        destruct (nat_eq_dec (S ieqv) (S (S neqv))).
+        ** eexists _. eexists _. exists eq_refl.
+          inversion e. subst ieqv. clear e.
+          unfold Common.l.
+          rewrite map_cons. unfold destination at 5.
+          assert
+            (Hfinal' :
+              equivocators_state_project final_choice
+                (last (map destination tr)
+                   (state_update (Common.equivocator_IM IM) is
+                      (eqv)
+                      (existT (fun n : nat => t (S n) -> vstate (IM (eqv)))
+                         (S neqv) bsi'))) =
+              last
+                (equivocators_state_project initial_choice'
+                   (state_update (Common.equivocator_IM IM) is
+                      (eqv)
+                      (existT (fun n : nat => t (S n) -> vstate (IM (eqv)))
+                         (S neqv) bsi')) :: map destination trX')
+                (equivocators_state_project
+                   (equivocators_choice_update initial_choice' eqv
+                      (Existing (IM (eqv)) idi true)) is)
+            ).
+          { rewrite unroll_last. subst bsi'. simpl in *. rewrite Hfinal.
+            rewrite (equivocators_state_project_state_update_eqv IM i0).
+            rewrite Heqv.
+            unfold projT1. unfold projT2.
+            reflexivity.
+          }
+          exists Hfinal'.
+          assert
+            (Hproper'' :
+            proper_equivocators_choice
+            (equivocators_choice_update initial_choice' eqv
+               (Existing (IM (eqv)) idi true)) is).
+          { intro eqv'. spec Hproper' eqv'.
+            unfold equivocators_choice_update.
+            destruct (decide (eqv' = eqv)).
+            - subst. rewrite state_update_eq in Hproper'.
+              rewrite equivocators_choice_update_eq.
+              rewrite Heqv in Hproper'.
+              simpl in *.
+              rewrite Hiseqv. simpl. lia.
+            - rewrite state_update_neq in Hproper' by congruence.
+              rewrite equivocators_choice_update_neq; assumption.
+          }
+          exists Hproper''.
+          constructor; [assumption|].
+          repeat split; [apply His; assumption|assumption|..].
+          --- remember equivocators_state_project as esp. simpl.
+            simpl in Hv. subst esp. unfold equivocators_state_project.
+            unfold Common.equivocators_state_project.
+            unfold equivocators_choice_update.
+            rewrite equivocators_choice_update_eq.
+            rewrite Hiseqv.
+            simpl in Hidi.
+            destruct (le_lt_dec (S neqv) idi); [lia|].
+            replace (of_nat_lt l0) with (of_nat_lt Hidi) in * by apply of_nat_ext.
+            clear l0.
+            assumption.
+          --- unfold equivocators_state_project.
+            rewrite equivocators_state_project_state_update_eqv.
+            rewrite Heqv. unfold projT1. unfold projT2.
+            destruct (le_lt_dec (S (S neqv)) (S neqv)); [lia|].
+            replace (of_nat_lt l) with (of_nat_lt Hproper_eqv) in * by apply of_nat_ext.
+            clear l.
+            replace (of_nat_lt l0) with (of_nat_lt Hproper_eqv) in * by apply of_nat_ext.
+            clear l0.
+            remember Common.equivocators_state_project as esp.
+            remember (of_nat_lt Hproper_eqv) as onl.
+            simpl.
+            rewrite  Heqesp.
+            unfold Common.equivocators_state_project at 1.
+            unfold equivocators_choice_update.
+            rewrite equivocators_choice_update_eq.
+            rewrite Hiseqv.
+            simpl in Hidi.
+            destruct (le_lt_dec (S neqv) idi); [lia|].
+            replace (of_nat_lt l) with (of_nat_lt Hidi) in * by apply of_nat_ext.
+            clear l. clear Hproject. subst. rewrite to_nat_of_nat.
+            destruct (nat_eq_dec (S neqv) (S neqv)); [|congruence].
+            simpl in *. rewrite Ht''.
+            f_equal.
+            apply functional_extensionality_dep_good.
+            intro eqvi.
+            destruct (decide (eqvi = eqv)).
+            +++ subst. repeat rewrite state_update_eq. reflexivity.
+            +++ repeat rewrite state_update_neq by assumption.
+              unfold  Common.equivocators_state_project.
+              destruct (decide (eqvi = eqv)); [congruence|].
+              rewrite equivocators_choice_update_neq; congruence.
+        ** eexists _. eexists _. exists eq_refl.
+          assert
+            (Hfinal' :
+              equivocators_state_project final_choice
+                (last (map destination tr)
+                   (state_update (Common.equivocator_IM IM) is
+                      (eqv)
+                      (existT (fun n0 : nat => t (S n0) -> vstate (IM (eqv)))
+                         (S neqv) bsi'))) =
+              last (map destination trX')
+                (equivocators_state_project
+                   (equivocators_choice_update initial_choice' eqv
+                      (Existing (IM (eqv)) ieqv false)) is)
+            ).
+          { subst bsi'. simpl in *. rewrite Hfinal.
+            rewrite (equivocators_state_project_state_update_eqv IM i0).
+            rewrite Heqv.
+            unfold projT1. unfold projT2.
+            f_equal.
+            apply functional_extensionality_dep_good.
+            destruct (le_lt_dec (S (S neqv)) ieqv); [lia|].
+            rewrite to_nat_of_nat.
+            destruct (nat_eq_dec ieqv (S neqv) ); [lia|].
+            intro i'. destruct (decide (i' = (eqv))).
+            - subst. rewrite state_update_eq.
+              unfold equivocators_state_project.
+              unfold Common.equivocators_state_project.
+              unfold equivocators_choice_update.
+              rewrite equivocators_choice_update_eq.
+              rewrite Hiseqv.
+              destruct (le_lt_dec (S neqv) ieqv); [lia|].
+              f_equal. apply of_nat_ext.
+            - rewrite state_update_neq by assumption.
+              unfold equivocators_state_project.
+              unfold Common.equivocators_state_project.
+              unfold equivocators_choice_update.
+              rewrite equivocators_choice_update_neq; congruence.
+          }
+          exists Hfinal'.
+          assert
+            (Hproper'' :
+            proper_equivocators_choice
+              (equivocators_choice_update initial_choice' eqv
+                 (Existing (IM (eqv)) ieqv false)) is).
+          { intro eqv'. spec Hproper' eqv'.
+            unfold equivocators_choice_update.
+            destruct (decide (eqv' = eqv)).
+            - subst. rewrite state_update_eq in Hproper'.
+              rewrite equivocators_choice_update_eq.
+              rewrite Heqv in Hproper'.
+              simpl in *.
+              rewrite Hiseqv. simpl. lia.
+            - rewrite state_update_neq in Hproper' by congruence.
+              rewrite equivocators_choice_update_neq; assumption.
+          }
+          exists Hproper''.
+          replace
+            (equivocators_state_project
+            (equivocators_choice_update initial_choice' eqv
+               (Existing (IM (eqv)) ieqv false)) is)
+            with
+            (equivocators_state_project initial_choice'
+            (state_update (Common.equivocator_IM IM) is
+               (eqv)
+               (existT (fun n : nat => t (S n) -> vstate (IM (eqv)))
+                  (S neqv) bsi')))
+          ; [assumption|].
+          unfold equivocators_state_project.
+          rewrite equivocators_state_project_state_update_eqv.
+          rewrite Heqv. unfold projT1. unfold projT2.
+          destruct (le_lt_dec (S (S neqv)) ieqv); [lia|].
+          replace (of_nat_lt l) with (of_nat_lt Hproper_eqv) in * by apply of_nat_ext.
+          clear l.
+          replace (of_nat_lt l0) with (of_nat_lt Hproper_eqv) in * by apply of_nat_ext.
+          clear l0.
+          apply functional_extensionality_dep_good.
+          intro i.
+          destruct (decide (i = eqv)).
+          --- subst. rewrite state_update_eq.
+            rewrite to_nat_of_nat.
+            destruct (nat_eq_dec ieqv (S neqv)); [congruence|].
+            unfold Common.equivocators_state_project.
+            unfold equivocators_choice_update.
+            rewrite equivocators_choice_update_eq.
+            rewrite Hiseqv.
+            destruct (le_lt_dec (S neqv) ieqv); [lia|].
+            f_equal. apply of_nat_ext.
+          --- rewrite state_update_neq by assumption.
+            unfold  Common.equivocators_state_project.
+            unfold equivocators_choice_update.
+            rewrite equivocators_choice_update_neq; congruence.
+      ++ inversion Ht'. subst. simpl_existT.
+        destruct (nat_eq_dec idi ieqv).
+        --- subst. simpl in Hidi.
+          replace (of_nat_lt l) with (of_nat_lt Hidi) in * by apply of_nat_ext.
+          clear l.
+          replace (of_nat_lt Hproper_eqv) with (of_nat_lt Hidi) in * by apply of_nat_ext.
+          clear Hproper_eqv.
+          rewrite eq_dec_if_true in * by reflexivity.
+          eexists _. eexists _. exists eq_refl.
+          rewrite map_cons. unfold destination at 5.
+          assert
+            (Hfinal' :
+              equivocators_state_project final_choice
+                (last (map destination tr)
+                   (state_update (Common.equivocator_IM IM) is
+                      (eqv)
+                      (existT (fun n : nat => t (S n) -> vstate (IM (eqv))) nsi'
+                         (fun j : t (S nsi') =>
+                          if eq_dec (of_nat_lt Hidi) j then si' else bseqv j)))) =
+              last
+                (equivocators_state_project initial_choice'
+                   (state_update (Common.equivocator_IM IM) is
+                      (eqv)
+                      (existT (fun n : nat => t (S n) -> vstate (IM (eqv))) nsi'
+                         (fun j : t (S nsi') =>
+                          if eq_dec (of_nat_lt Hidi) j then si' else bseqv j)))
+                 :: map destination trX')
+                (equivocators_state_project
+                   (equivocators_choice_update initial_choice' eqv
+                      (Existing (IM (eqv)) ieqv false)) is)
+            ).
+          { rewrite unroll_last. simpl in *. rewrite Hfinal.
+            rewrite (equivocators_state_project_state_update_eqv IM i0).
+            rewrite Heqv.
+            unfold projT1. unfold projT2.
+            reflexivity.
+          }
+          exists Hfinal'.
+          assert
+            (Hproper'' : proper_equivocators_choice
+            (equivocators_choice_update initial_choice' eqv
+               (Existing (IM (eqv)) ieqv false)) is).
+          { intro eqv'. spec Hproper' eqv'.
+            unfold equivocators_choice_update.
+            destruct (decide (eqv' = eqv)).
+            - subst. rewrite state_update_eq in Hproper'.
+              rewrite equivocators_choice_update_eq.
+              rewrite Heqv in Hproper'.
+              simpl in *.
+              rewrite Hiseqv. simpl. lia.
+            - rewrite state_update_neq in Hproper' by congruence.
+              rewrite equivocators_choice_update_neq; assumption.
+          }
+          exists Hproper''.
+          constructor; [assumption|].
+          repeat split; [apply His; assumption| assumption| |].
+          +++ remember equivocators_state_project as esp. simpl.
+            simpl in Hv. subst esp. unfold equivocators_state_project.
+            unfold Common.equivocators_state_project.
+            unfold equivocators_choice_update.
+            rewrite equivocators_choice_update_eq.
+            rewrite Hiseqv.
+            simpl in Hidi.
+            destruct (le_lt_dec (S nsi') ieqv); [lia|].
+            replace (of_nat_lt l) with (of_nat_lt Hidi) in * by apply of_nat_ext.
+            clear l.
+            assumption.
+          +++ unfold equivocators_state_project.
+            rewrite equivocators_state_project_state_update_eqv.
+            rewrite Heqv. unfold projT1. unfold projT2.
+            destruct (le_lt_dec (S nsi') ieqv); [lia|].
+            replace (of_nat_lt l) with (of_nat_lt Hidi) in * by apply of_nat_ext.
+            clear l.
+            remember Common.equivocators_state_project as esp.
+            remember (of_nat_lt Hidi) as onl.
+            simpl.
+            rewrite  Heqesp.
+            unfold Common.equivocators_state_project at 1.
+            unfold equivocators_choice_update.
+            rewrite equivocators_choice_update_eq.
+            rewrite Hiseqv.
+            destruct (le_lt_dec (S nsi') ieqv); [lia|].
+            replace (of_nat_lt l) with (of_nat_lt Hidi) in * by apply of_nat_ext.
+            clear l. clear Hproject. subst. rewrite eq_dec_if_true by reflexivity.
+            simpl in *. rewrite Ht''.
+            f_equal.
+            apply functional_extensionality_dep_good.
+            intro eqvi.
+            destruct (decide (eqvi = eqv)).
+            *** subst. repeat rewrite state_update_eq. reflexivity.
+            *** repeat rewrite state_update_neq by  assumption.
+              unfold  Common.equivocators_state_project.
+              destruct (decide (eqvi = eqv)); [congruence|].
+              rewrite equivocators_choice_update_neq; congruence.
+        --- eexists _. eexists _. exists eq_refl.
+          assert
+            (Hfinal' :
+              equivocators_state_project final_choice
+                (last (map destination tr)
+                   (state_update (Common.equivocator_IM IM) is
+                      (eqv)
+                      (existT (fun n0 : nat => t (S n0) -> vstate (IM (eqv)))
+                         nsi' bsi'))) =
+              last (map destination trX')
+                (equivocators_state_project
+                   (equivocators_choice_update initial_choice' eqv
+                      (Existing (IM (eqv)) ieqv false)) is)
+            ).
+          { subst bsi'. simpl in *. rewrite Hfinal.
+            rewrite (equivocators_state_project_state_update_eqv IM i0).
+            rewrite Heqv.
+            unfold projT1. unfold projT2.
+            f_equal.
+            apply functional_extensionality_dep_good.
+            destruct (le_lt_dec (S nsi') ieqv); [lia|].
+            destruct (eq_dec (of_nat_lt Hidi) (of_nat_lt l0))
+            ; [apply (f_equal to_nat) in e; repeat rewrite to_nat_of_nat in e; congruence|].
+            intro i'. destruct (decide (i' = (eqv))).
+            - subst. rewrite state_update_eq.
+              unfold equivocators_state_project.
+              unfold Common.equivocators_state_project.
+              unfold equivocators_choice_update.
+              rewrite equivocators_choice_update_eq.
+              rewrite Hiseqv.
+              destruct (le_lt_dec (S nsi') ieqv); [lia|].
+              f_equal. apply of_nat_ext.
+            - rewrite state_update_neq by assumption.
+              unfold equivocators_state_project.
+              unfold Common.equivocators_state_project.
+              unfold equivocators_choice_update.
+              rewrite equivocators_choice_update_neq; congruence.
+          }
+          exists Hfinal'.
+          assert
+            (Hproper'' :
+            proper_equivocators_choice
+              (equivocators_choice_update initial_choice' eqv
+                 (Existing (IM (eqv)) ieqv false)) is).
+          { intro eqv'. spec Hproper' eqv'.
+            unfold equivocators_choice_update.
+            destruct (decide (eqv' = eqv)).
+            - subst. rewrite state_update_eq in Hproper'.
+              rewrite equivocators_choice_update_eq.
+              rewrite Heqv in Hproper'.
+              simpl in *.
+              rewrite Hiseqv. simpl. lia.
+            - rewrite state_update_neq in Hproper' by congruence.
+              rewrite equivocators_choice_update_neq; assumption.
+          }
+          exists Hproper''.
+          replace
+            (equivocators_state_project
+            (equivocators_choice_update initial_choice' eqv
+               (Existing (IM (eqv)) ieqv false)) is)
+            with
+            (equivocators_state_project initial_choice'
+            (state_update (Common.equivocator_IM IM) is
+               (eqv)
+               (existT (fun n : nat => t (S n) -> vstate (IM (eqv)))
+                  nsi' bsi')))
+          ; [assumption|].
+          unfold equivocators_state_project.
+          rewrite equivocators_state_project_state_update_eqv.
+          rewrite Heqv. unfold projT1. unfold projT2.
+          destruct (le_lt_dec (S nsi') ieqv); [lia|].
+          replace (of_nat_lt l0) with (of_nat_lt Hproper_eqv) in * by apply of_nat_ext.
+          clear l0.
+          apply functional_extensionality_dep_good.
+          intro i.
+          destruct (decide (i = eqv)).
+          +++ subst. rewrite state_update_eq.
+            rewrite eq_dec_if_false.
+            *** unfold Common.equivocators_state_project.
+              unfold equivocators_choice_update.
+              rewrite equivocators_choice_update_eq.
+              rewrite Hiseqv.
+              destruct (le_lt_dec (S nsi') ieqv); [lia|].
+              f_equal. apply of_nat_ext.
+            *** intro contra. elim n. apply (f_equal to_nat) in contra.
+              repeat rewrite to_nat_of_nat in contra. inversion contra. reflexivity.
+          +++ rewrite state_update_neq by assumption.
+            unfold  Common.equivocators_state_project.
+            unfold equivocators_choice_update.
+            rewrite equivocators_choice_update_neq; congruence.
+Qed.
+
+End equivocators_composition_projections.
