VLSM/Equivocators/MergeProjections.v
@@ -130,15 +130,15 @@ Lemma projection_traces_replace_one_length
 Proof.
   unfold projection_traces_replace_one.
   unfold projection_traces.
-  rewrite map_option_length; try apply fin_t_listing_length.
+  rewrite map_option_length; [apply fin_t_listing_length|].
   apply Forall_forall.
   intros nj Hnj.
   unfold preloaded_protocol_equivocator_vlsm_trace_oproject_update.
   unfold equivocator_projection_update.
   destruct (Fin.eq_dec ni nj).
-  - rewrite eq_dec_if_true; try assumption.
-    intro contra. discriminate contra.
-  - rewrite eq_dec_if_false; try assumption.
+  - rewrite eq_dec_if_true by assumption.
+    congruence.
+  - rewrite eq_dec_if_false by assumption.
     unfold preloaded_protocol_equivocator_vlsm_trace_oproject.
     destruct (to_nat nj) as [j Hj] eqn:Heqnj.
     destruct
@@ -146,10 +146,10 @@ Proof.
       as [trX [di [Hproject Hdi]]].
     rewrite Hproject.
     destruct di as [sn | i fi].
-    + intro contra. discriminate contra.
+    + congruence.
     + destruct Hdi as [Hi [HlstX [HtrX]]].
-      destruct (le_lt_dec (S (projT1 is)) i). { lia. }
-      intro contra. discriminate contra.
+      destruct (le_lt_dec (S (projT1 is)) i); [lia|].
+      congruence.
 Qed.
 
 Context
